cleanups, variance labled trees

SortEmbeddings.v
@@ -5,6 +5,9 @@ Require Import SigmaAlgebra.
 Require Import CombinatoryLogic.
 Require Import IntersectionTypes.
 Require Import CombinatoryLogicAlgebra.
+Require Import FiniteSubstitutionSpace.
+Require Import ComputationalPathLemma.
+Require Import VarianceLabeledTree.
 Require Import Cantor.
 
 Module Type FiniteCountableSignatureSpec <: SignatureSpec.
@@ -266,22 +269,368 @@ Module Type ProperConstantEmbedding
        unembedApply := Proper.unembedApply |}.       
 End ProperConstantEmbedding.
 
-(*
-Module ConstantSortSymbolSpecification(Signature: ConstantSortSignature): SignatureSymbolSpecification(Signature).
-  Module Type Spec <: SignatureSymbolSpecification(Signature).
-    Definition ConstructorSymbol := Signature.Sort EmptySet.
-    Definition constructorArity: ConstructorSymbol -> nat := fun _ => 0.
-    Definition ConstructorTaxonomy : ConstructorSymbol -> ConstructorSymbol -> Prop := Signature.subsorts.
-    Definition CTPreorder : PreOrder ConstructorTaxonomy := Signature.subsorts_pre.
-    Definition ConstructorSymbol_eq_dec:
-      forall (C1 C2: ConstructorSymbol), {C1 = C2} + {C1 <> C2} := Signature.Sort_eq_dec.
+Module Type ConstantFiniteWellFormedPredicate
+       (Import SigSpec: CountableClosedSortSignatureSpec)
+       (Import MakeSignature: MakeClosedSortCLSignature(SigSpec))
+       (Import Types: IntersectionTypes(MakeSignature.Signature))
+<: FiniteWellFormedPredicate(MakeSignature.Signature)(Types)
+<: DecidableWellFormedPredicate(MakeSignature.Signature)(Types).
+  Definition WellFormed: Substitution -> Prop := fun S => forall alpha, S alpha = omega.
+  Definition SubstitutionSpace : Set := unit.
+  Definition SubstitutionSpace_sound: SubstitutionSpace -> { S : Substitution | WellFormed S } :=
+    fun _ => exist _ (fun _ => omega) (fun alpha => eq_refl).
+  Definition SubstitutionSpace_complete: { S : Substitution | WellFormed S } -> SubstitutionSpace :=
+    fun _ => tt.
+  Lemma SubstitutionSpace_eq:
+    forall WFS alpha, proj1_sig (SubstitutionSpace_sound (SubstitutionSpace_complete WFS)) alpha =
+                 proj1_sig WFS alpha.
+  Proof.
+    intros WFS alpha; simpl.
+    rewrite (proj2_sig WFS alpha).
+    reflexivity.
+  Qed.
+  Instance SubstitutionSpace_finite: Finite SubstitutionSpace :=
+    {| cardinality := 1;
+       toFin := fun _ => Fin.F1;
+       fromFin := fun _ => tt;
+       fromToFin_id := fun x => match x with | tt => eq_refl end |}.
+  Lemma WF_dec: forall S, { WellFormed S } + { ~ WellFormed S }.
+  Proof.
+    intro S; left; intro alpha.
+    contradiction.
+  Qed.
+
+  Lemma WF_ext: forall S S', (forall alpha, S alpha = S' alpha) -> WellFormed S -> WellFormed S'.
+  Proof.
+    intros S S' S_eq WF_S.
+    intro alpha.
+    rewrite <- (S_eq alpha).
+    apply WF_S.
+  Qed.
+   
+End ConstantFiniteWellFormedPredicate.                  
+
+
+
+(* Trees *)
+Module Type TreeSpec.
+  Parameter Label: Set.
+  Parameter Var: Set.
+  Parameter LOrder: Label -> Label -> Prop.
+
+  Declare Instance Info: LabelInfo Label.
+  Declare Instance LOrder_pre: PreOrder LOrder.
+
+  Parameter Operation: Set.
+  Parameter WellFormed: (Var -> VLTree Label EmptySet) -> Prop.
+  Declare Instance Sigma: Signature (VLTree Label) Var Operation.
+
+  Parameter Var_eq_dec:  forall (alpha beta: Var), { alpha = beta } + { alpha <> beta }.
+  Parameter Label_eq_dec: forall (l1 l2: Label), { l1 = l2 } + { l1 <> l2 }.  
+End TreeSpec.
+(* TODO:
+
+Module Type TreeSignatureSpec(Import Trees: TreeSpec) <: FiniteCountableSignatureSpec.
+  Definition Sort: Set -> Set := VLTree Label.
+  Definition Var: Set := Trees.Var.
+  Definition Operation: Set := Trees.Operation.
+  Definition WellFormed: (Var -> Sort EmptySet) -> Prop := Trees.WellFormed.
+  Instance SigSpec: SignatureSpecification Sort Var Operation := SigSpec.SigSpec.
   
-    Definition ConstructorTaxonomy_dec:
-      forall (C1 C2: ConstructorSymbol), { ConstructorTaxonomy C1 C2 } + { ConstructorTaxonomy C1 C2 -> False } :=
-      Signature.subsorts_dec.
-    Definition VariableSymbol := Signature.Var.
-    Definition CombinatorSymbol: Set := Operation.
-  End Spec.
+  Declare Instance SigSpec: SignatureSpecification Sort Var Operation.
+End SignatureSpec.
+
+
+Module Type TreeSortCLSignature(SigSpec: FiniteCountableSignatureSpec) <: CompatibleCLSignature.
+  Definition Sort: Set -> Set := SigSpec.Sort.
+  Definition Var: Set := SigSpec.Var.
+  Definition Operation: Set := SigSpec.Operation.
+  Definition WellFormed: (Var -> Sort EmptySet) -> Prop := SigSpec.WellFormed.
+  Instance SigSpec: SignatureSpecification Sort Var Operation := SigSpec.SigSpec.
+  
+  Definition ConstructorSymbol := (unit + Sort EmptySet)%type.
+  Definition VariableSymbol := Var.
+  Definition CombinatorSymbol := Operation.
+  Definition VariableSymbol_eq_dec := Var_eq_dec.
+  Module ConstructorDefs.
+    Definition ConstructorTaxonomy: ConstructorSymbol -> ConstructorSymbol -> Prop :=
+      fun c1 c2 =>
+        match c1 with
+        | inr c1 =>
+          match c2 with
+          | inr c2 => subsorts c1 c2
+          | _ => False
+          end
+        | inl tt =>
+          match c2 with
+          | inl tt => True
+          | inr _ => False
+          end
+        end.
+    Lemma ConstructorTaxonomy_reflexive: Reflexive ConstructorTaxonomy.
+    Proof.
+      intro x.
+      destruct x as [ [ ] | s ].
+      - simpl; trivial.
+      - simpl.
+        generalize (subsorts_pre).
+        intro presub.
+        reflexivity.
+    Qed.
+
+    Lemma ConstructorTaxonomy_transitive: Transitive ConstructorTaxonomy.
+    Proof.
+      intros x y z.
+      destruct x as [ [] | x ]; destruct y as [ [] | y ]; destruct z as [ [] | z ];
+        intros xy yz;
+        try solve [ contradiction | trivial ].
+      generalize (subsorts_pre); intro presub.
+      simpl.
+      transitivity y; assumption.
+    Qed.
+
+    Lemma ConstructorTaxonomy_eq_dec: forall (c1 c2: ConstructorSymbol), { c1 = c2 } + { c1 <> c2 }.
+    Proof.
+      intros c1 c2.
+      destruct c1 as [ [] | c1 ]; destruct c2 as [ [] | c2 ];
+        try solve [ left; reflexivity | right; intro devil; inversion devil ].
+      generalize (SigSpec).
+      intro sigspec.
+      destruct (Sort_eq_dec c1 c2);
+        [ left; apply f_equal; assumption
+        | right; intro devil; inversion devil; contradiction ].
+    Qed.
+
+    Lemma ConstructorTaxonomy_dec: forall c1 c2, { ConstructorTaxonomy c1 c2 } + { ConstructorTaxonomy c1 c2 -> False }.
+    Proof.
+      intros c1 c2.
+      destruct c1 as [ [] | ]; destruct c2 as [ [] | ];
+        try solve [ left; reflexivity | right; intro; assumption ].
+      apply subsorts_dec.
+    Qed.
+
+    Definition constructorSymbolToNat (c: ConstructorSymbol): nat :=
+      match c with
+      | inl tt => cantor_sum (inl 0)
+      | inr c => cantor_sum (inr (toNat c))
+      end.
+    Definition natToConstructorSymbol (n: nat): ConstructorSymbol :=
+      match cantor_sum_inv n with
+      | inl _ => inl tt
+      | inr n => inr (fromNat n)
+      end.
+    Lemma fromToConstructorSymbol_id: forall c, natToConstructorSymbol (constructorSymbolToNat c) = c.
+    Proof.
+      intro c.
+      destruct c as [ [] | c ].
+      - reflexivity.
+      - unfold constructorSymbolToNat.
+        unfold natToConstructorSymbol.
+        rewrite cantor_sum_inj.
+        rewrite fromTo_id.
+        reflexivity.
+    Qed.
+  End ConstructorDefs.
     
-  Include SignatureSymbolSpecification(Signature) <+ Spec.
+  Definition Symbols: ConstructorSpecification ConstructorSymbol :=
+    {| constructorArity := fun c => match c with | inl _ => 1 | inr _ => 0 end;
+       ConstructorTaxonomy := ConstructorDefs.ConstructorTaxonomy;        
+       CTPreorder :=
+         {| PreOrder_Reflexive := ConstructorDefs.ConstructorTaxonomy_reflexive;
+            PreOrder_Transitive := ConstructorDefs.ConstructorTaxonomy_transitive |};
+       ConstructorSymbol_eq_dec := ConstructorDefs.ConstructorTaxonomy_eq_dec;
+       ConstructorTaxonomy_dec := ConstructorDefs.ConstructorTaxonomy_dec |}.
+  Instance ConstructorSymbol_countable: Countable ConstructorSymbol :=
+    {| toNat := ConstructorDefs.constructorSymbolToNat;
+       fromNat := ConstructorDefs.natToConstructorSymbol;
+       fromTo_id := ConstructorDefs.fromToConstructorSymbol_id |}.
+  Instance Variables_finite: Finite VariableSymbol := SigSpec.Vars_finite.
+  Definition ClosedSortsInhabited: Sort EmptySet := fromNat 0.
+  Definition OpenSortsInhabited: Sort Var := SigSpec.OpenSortsInhabited.
+  Definition BlackBox : ConstructorSymbol := inl tt.
+  Lemma BlackBoxArity: @constructorArity _ Symbols BlackBox = 1.
+  Proof.
+    reflexivity.
+  Qed.
+End SortConstructorCLSignature.
+
+Module Type CountableClosedSortSignatureSpec.
+  Include SignatureSpec with Definition Var := EmptySet.
+  Declare Instance ClosedSortsCountable: Countable (Sort EmptySet).
+  Parameter applySubst_eq: forall S s, applySubst S s = s.
+End CountableClosedSortSignatureSpec.
+
+Module Type FiniteCountableFromCountableClosedSortSignatureSpec
+       (SigSpec: CountableClosedSortSignatureSpec) <: FiniteCountableSignatureSpec.
+  Definition Sort: Set -> Set := SigSpec.Sort.
+  Definition Var: Set := SigSpec.Var.
+  Definition Operation: Set := SigSpec.Operation.
+  Definition WellFormed: (Var -> Sort EmptySet) -> Prop := SigSpec.WellFormed.
+  Instance SigSpec: SignatureSpecification Sort Var Operation := SigSpec.SigSpec.
+  Instance ClosedSortsCountable: Countable (Sort EmptySet) := SigSpec.ClosedSortsCountable.
+  Instance Vars_finite: Finite Var :=
+    {| cardinality := 0;
+       toFin := fun devil => False_rect _ devil;
+       fromFin := fun devil =>
+                    match devil in Fin.t n return 0 = n -> EmptySet with
+                    | Fin.F1 =>
+                      fun devil' =>
+                        match devil' in _ = n return match n with | 0 => True | _ => False end with
+                        | eq_refl => I
+                        end  
+                    | Fin.FS _ =>
+                      fun devil' =>
+                        match devil' in _ = n return match n with | 0 => True | _ => False end with
+                        | eq_refl => I
+                        end
+                    end eq_refl;
+       fromToFin_id := fun devil => False_rect _ devil |}.
+  Definition OpenSortsInhabited: Sort Var := fromNat 0.
+End FiniteCountableFromCountableClosedSortSignatureSpec.
+
+Module Type MakeClosedSortCLSignature(SigSpec: CountableClosedSortSignatureSpec).
+  Declare Module SigSpec' : FiniteCountableFromCountableClosedSortSignatureSpec(SigSpec).
+  Declare Module Signature : SortConstructorCLSignature(SigSpec').
+End MakeClosedSortCLSignature.
+
+
+Module Type ProperConstantEmbedding
+       (Import SigSpec: CountableClosedSortSignatureSpec)
+       (Import MakeSignature: MakeClosedSortCLSignature(SigSpec))
+       (Import Types: IntersectionTypes(MakeSignature.Signature))
+<: WithProperEmbedding(MakeSignature.Signature)(Types).
+  
+  Module Embedding : SortEmbedding(Signature)(Types).
+    Include SortEmbedding(Signature)(Types).
+  End Embedding.
+
+  Import Embedding.
+
+  Module Proper.
+    Import Signature.
+    Definition embedS (s: Sort EmptySet) := ConstScheme (inr s) (nil _).
+    Definition unembedS (ts: TypeScheme (VariableSymbol := EmptySet)): Sort EmptySet :=
+      match ts with
+      | Skeleton (PT_Const (inr C) _) => C
+      | _ => OpenSortsInhabited
+      end.
+
+    Instance ClosedEmbedding : Embedding EmptySet :=
+      {| embed := embedS; unembed := unembedS |}.
+
+    Lemma injectivity: forall (s: Sort EmptySet), unembed (embed s) = s.
+    Proof.
+      intro; reflexivity.
+    Qed.
+
+    Instance ClosedInjectiveEmbedding: InjectiveEmbedding EmptySet :=
+      {| Embed := ClosedEmbedding; unembedEmbed := injectivity |}.
+
+    Lemma embed_respectful: forall s s', subsorts s s' -> freeze (embed s) <= freeze (embed s').
+    Proof.
+      intros s s' s_le.
+      apply (ST_Ax (inr s) (inr s') eq_refl); [ assumption | apply Forall2_nil ].
+    Qed.
+
+    Lemma unembed_respectful: forall (sigma tau: IntersectionType),
+        (exists s, sigma = freeze (embed s)) -> (exists s, tau = freeze (embed s)) ->
+        sigma <= tau -> subsorts (unembed (unfreeze sigma)) (unembed (unfreeze tau)).
+    Proof.
+      intros sigma tau ex_l ex_r.
+      destruct ex_l as [ s sigma_eq ].
+      destruct ex_r as [ s' tau_eq ].
+      rewrite sigma_eq.
+      rewrite tau_eq.
+      rewrite freezeUnfreeze.
+      rewrite freezeUnfreeze.
+      intro sigma_le.
+      simpl in sigma_le.
+      generalize (CI_complete _ _ _ sigma_le).
+      intro sigma_le'.
+      inversion sigma_le'.
+      rewrite injectivity.
+      rewrite injectivity.
+      assumption.
+    Qed.
+
+    Lemma embed_Path: forall s, Path (freeze (embed s)).
+    Proof.
+      intros.
+      apply Path_Const.
+      apply PathArgs_nil.
+    Qed.
+
+    Lemma embedApply: forall S s, freeze (embed (applySubst S s)) = Apply (embedSubst S) (embed s).
+    Proof.
+      intros S s.
+      simpl.
+      rewrite applySubst_eq.
+      reflexivity.
+    Qed.
+
+    Lemma unembedApply: forall S tau,
+        (exists s, tau = embed s) ->
+        Apply S tau = freeze (embed (applySubst (unembedSubst S) (unembed tau))).
+    Proof.
+      intros S tau ex_prf.
+      simpl.
+      rewrite applySubst_eq.
+      destruct ex_prf as [ s tau_eq ].
+      simpl embed in tau_eq.
+      unfold embedS in tau_eq.
+      rewrite tau_eq.
+      simpl.
+      reflexivity.
+    Qed.
+  End Proper.
+  Instance ProperlyEmbedded: ProperEmbedding :=
+    {| EmbedClosed := Proper.ClosedInjectiveEmbedding;
+       EmbedOpen := Proper.ClosedInjectiveEmbedding;
+       embed_respectful := Proper.embed_respectful;
+       unembed_respectful := Proper.unembed_respectful;
+       embed_Path := Proper.embed_Path;
+       embedApply := Proper.embedApply;
+       unembedApply := Proper.unembedApply |}.       
+End ProperConstantEmbedding.
+
+Module Type ConstantFiniteWellFormedPredicate
+       (Import SigSpec: CountableClosedSortSignatureSpec)
+       (Import MakeSignature: MakeClosedSortCLSignature(SigSpec))
+       (Import Types: IntersectionTypes(MakeSignature.Signature))
+<: FiniteWellFormedPredicate(MakeSignature.Signature)(Types)
+<: DecidableWellFormedPredicate(MakeSignature.Signature)(Types).
+  Definition WellFormed: Substitution -> Prop := fun S => forall alpha, S alpha = omega.
+  Definition SubstitutionSpace : Set := unit.
+  Definition SubstitutionSpace_sound: SubstitutionSpace -> { S : Substitution | WellFormed S } :=
+    fun _ => exist _ (fun _ => omega) (fun alpha => eq_refl).
+  Definition SubstitutionSpace_complete: { S : Substitution | WellFormed S } -> SubstitutionSpace :=
+    fun _ => tt.
+  Lemma SubstitutionSpace_eq:
+    forall WFS alpha, proj1_sig (SubstitutionSpace_sound (SubstitutionSpace_complete WFS)) alpha =
+                 proj1_sig WFS alpha.
+  Proof.
+    intros WFS alpha; simpl.
+    rewrite (proj2_sig WFS alpha).
+    reflexivity.
+  Qed.
+  Instance SubstitutionSpace_finite: Finite SubstitutionSpace :=
+    {| cardinality := 1;
+       toFin := fun _ => Fin.F1;
+       fromFin := fun _ => tt;
+       fromToFin_id := fun x => match x with | tt => eq_refl end |}.
+  Lemma WF_dec: forall S, { WellFormed S } + { ~ WellFormed S }.
+  Proof.
+    intro S; left; intro alpha.
+    contradiction.
+  Qed.
+
+  Lemma WF_ext: forall S S', (forall alpha, S alpha = S' alpha) -> WellFormed S -> WellFormed S'.
+  Proof.
+    intros S S' S_eq WF_S.
+    intro alpha.
+    rewrite <- (S_eq alpha).
+    apply WF_S.
+  Qed.
+   
+End ConstantFiniteWellFormedPredicate.                  
 *)
