CombinatoryLogicAlgebra.v
@@ -131,7 +131,578 @@ Module Type WithProperEmbedding(SigSpec: CompatibleCLSignature)(Types: Intersect
   Declare Instance ProperlyEmbedded: ProperEmbedding.
 End WithProperEmbedding.
 
+
+
+Module CombinatoryLogicAlgebra
+       (Import SigSpec: CompatibleCLSignature)
+       (Import Types: IntersectionTypes(SigSpec))
+       (Import Terms: Terms(SigSpec))
+       (Import ProperEmbedding: WithProperEmbedding(SigSpec)(Types))
+       (Import TypesCountable: CountableTypes(SigSpec)(Types))
+       (Import WF: DecidableWellFormedPredicate(SigSpec)(Types))
+       (Import CL: CombinatoryLogic(SigSpec)(Types)(Terms)(WF))
+       (Import CPL: ComputationalPathLemma(SigSpec)(Types)(Terms)(TypesCountable)(WF)(CL))
+       (Import Alg: Algebraic(SigSpec)).
+  
+  Definition blackBoxEmbedOpen (s: Sort SigSpec.Var): TypeScheme (VariableSymbol := SigSpec.Var) :=
+    ConstScheme BlackBox (rew <- BlackBoxArity in cons _ (embed s) _ (nil _)).
+
+  Definition blackBoxEmbed (s: Sort EmptySet): IntersectionType :=
+    freeze (Skeleton (PT_Const BlackBox (rew <- BlackBoxArity in cons _ (embed s) _ (nil _)))).
+
+  Definition Gamma (c: Operation) :=
+    (fix Gamma_rec n dom :=
+       match dom with
+       | nil _ => blackBoxEmbedOpen (range c)
+       | cons _ param _ params =>
+         ArrowScheme (blackBoxEmbedOpen param) (Gamma_rec _ params)
+       end) _ (domain c).
+  
+  Lemma Gamma_paths:
+    forall (c: Operation) (S: SigSpec.Var -> Sort EmptySet),
+      Path (Apply (embedSubst S) (Gamma c)).
+  Proof.
+    intros c S.
+    unfold Gamma.
+    induction (domain c).
+    - unfold blackBoxEmbedOpen.
+      apply Path_Const.
+      simpl.
+      rewrite BlackBoxArity.
+      simpl.
+      apply PathArgs_cons_arg.
+      fold (Apply).
+      rewrite <- embedApply.
+      apply embed_Path.
+    - apply Path_Arr.
+      assumption.
+  Qed.
+
+  Lemma source_count_eq : forall S op, src_count (Apply (embedSubst S) (Gamma op)) = arity op.
+  Proof.
+    intros S op.
+    unfold Gamma.
+    generalize (arity op) (domain op).
+    intros arity domain.
+    induction domain as [ | ? ? ? IH ].
+    - reflexivity.
+    - simpl.
+      rewrite IH.
+      reflexivity.
+  Qed. 
+
+  Definition Carrier s := { M : Term | CL Gamma M (blackBoxEmbed s) }.
+
+  Definition ProjectTerms: forall S n (args: t (Sort SigSpec.Var) n),
+      F_args Carrier S args -> t Term n :=
+    fun S n args f => 
+      map (fun k => proj1_sig ((F_args_nth _ _ _ f) k)) (positions n).
+
+  Lemma blackBoxEmbed_nth:
+    forall op S k (src_count_eq: src_count (Apply (embedSubst S) (Gamma op)) = arity op),
+      blackBoxEmbed (applySubst S (nth (domain op) (rew <- eq_sym src_count_eq in k))) =
+      nth
+        (fst
+           (split_path (Apply (embedSubst S) (Gamma op)) (src_count (Apply (embedSubst S) (Gamma op)))
+                       (le_n (src_count (Apply (embedSubst S) (Gamma op)))))) k.
+  Proof.
+    intros op S k src_count_eq.
+    generalize (le_n (src_count (Apply (embedSubst S) (Gamma op)))).
+    revert k.
+    generalize src_count_eq.
+    match goal with
+    | [ |- ?tgt ] =>
+      apply (fun x =>
+               rew <- [fun n =>
+                        forall (src_count_eq: n = arity op)
+                          (k: Fin.t n)
+                          (prf: (n <= src_count (Apply (embedSubst S) (Gamma op)))%nat),
+                          blackBoxEmbed (applySubst S (nth (domain op) (rew <- [Fin.t] eq_sym src_count_eq in k))) =
+                          nth (fst (split_path (Apply (embedSubst S) (Gamma op)) n prf)) k]
+                   (src_count_eq) in x)
+    end.
+    clear src_count_eq.
+    intros src_count_eq k prf.
+    unfold eq_rect_r.
+    rewrite <- (eq_rect_eq_dec (Nat.eq_dec) _ _ (eq_sym _)).
+    clear src_count_eq.
+    apply (Forall2_nth (fun x y => blackBoxEmbed (applySubst S x) = y)
+                       (domain op)
+                       (fst (split_path (Apply (embedSubst S) (Gamma op)) (arity op) prf))).
+    clear k.
+    revert prf.
+    unfold Gamma.
+    induction (domain op) as [ | ? ? ? IH ].
+    - intros; apply Forall2_nil.
+    - intro prf. 
+      apply Forall2_cons.
+      + unfold blackBoxEmbed.
+        unfold blackBoxEmbedOpen.
+        simpl.
+        apply f_equal.
+        rewrite BlackBoxArity.
+        simpl.
+        rewrite embedApply.
+        reflexivity.
+      + apply IH.
+  Qed.
+  
+  Definition CL_Algebra:
+      (forall S, SigSpec.WellFormed S -> WF.WellFormed (embedSubst S)) ->
+      SigmaAlgebra Carrier.
+  Proof.
+    unfold SigmaAlgebra.
+    intros WF_transport s Fs.
+    destruct Fs as [ op S WF_S args tgt_le ].
+    assert (opty : CL Gamma (Symbol op) (Apply (embedSubst S) (Gamma op))).
+    { apply CL_Var.
+      apply WF_transport; assumption. }
+    generalize (source_count_eq S op).
+    intro source_count_eq.
+    assert (args' :
+              { Ns: t Term (src_count (Apply (embedSubst S) (Gamma op)))
+              | Forall2 (CL Gamma) Ns (fst (split_path (Apply (embedSubst S) (Gamma op))
+                                                       (src_count (Apply (embedSubst S) (Gamma op)))
+                                                       (le_n _))) }).
+    { exists (rew <- source_count_eq in ProjectTerms _ _ _ args).
+      apply nth_Forall2.
+      unfold eq_rect_r.
+      intro k.
+      assert (rew_ext:
+                (rew [fun n => t Term n] eq_sym source_count_eq in (ProjectTerms S (arity op) (domain op) args)) =
+                rew [t Term] eq_sym source_count_eq in (ProjectTerms S (arity op) (domain op) args)).
+      { rewrite <- (eq_sym source_count_eq).
+        simpl.
+        reflexivity. }
+      rewrite rew_ext.
+      rewrite (nth_k (eq_sym source_count_eq) (ProjectTerms S (arity op) (domain op) args) k).
+      unfold ProjectTerms.
+      rewrite (nth_map _ _ _ _ eq_refl).
+      rewrite (positions_spec).
+      destruct (F_args_nth _ _ _ args (rew <- [Fin.t] eq_sym source_count_eq in k)) as [ M proof ].        
+      simpl.
+      rewrite <- (blackBoxEmbed_nth _ _ _ source_count_eq).
+      assumption. }
+    clear args.
+    assert (tgt_le':
+              snd (split_path (Apply (embedSubst S) (Gamma op))
+                              (src_count (Apply (embedSubst S) (Gamma op)))
+                              (le_n _)) <= blackBoxEmbed s).
+    { unfold blackBoxEmbed.
+      simpl freeze.
+      unfold Gamma.
+      clear args'.
+      generalize (domain op).
+      rewrite <- source_count_eq.
+      clear source_count_eq.
+      intro domain.
+      induction domain as [ | ? ? ? IH ].
+      - simpl.
+        apply (ST_Ax _ _ eq_refl); [ reflexivity | ].
+        rewrite BlackBoxArity.
+        apply Forall2_cons; [ | apply Forall2_nil ].
+        rewrite <- embedApply.
+        apply embed_respectful.
+        assumption.
+      - simpl.
+        match goal with
+        | [ |- (snd (split_path _ _ ?prfSx) <= _)] =>
+          rewrite (split_path_proof_invariant _ _ _ prfSx) in IH
+        end.
+        exact IH. }
+    eexists.
+    eapply CL_ST; [ | apply tgt_le' ].
+    eapply CL_ApplyPath.
+    - apply Gamma_paths. 
+    - eassumption.
+    - exact (proj2_sig args').
+  Defined.
+
+  Lemma unembedApply_c: forall S c,
+      Apply (embedSubst (unembedSubst S)) (Gamma c) =
+      Apply S (Gamma c).
+  Proof.
+    intros S c.
+    unfold Gamma.
+    induction (domain c) as [ | ? ? ? IH ].
+    - unfold blackBoxEmbedOpen.
+      simpl Apply.
+      apply f_equal.
+      rewrite BlackBoxArity.
+      simpl.
+      match goal with
+      |[|- cons _ ?lhs _ _ = cons _ ?rhs _ _] =>
+       assert (s_eq: lhs = rhs)
+      end.
+      { match goal with
+        |[|- _ = Apply S ?erc ] =>
+         assert (ex_s: exists s, erc = embed s); [ eexists; reflexivity | ];
+           rewrite (unembedApply S _ ex_s)
+        end.
+        rewrite <- embedApply.
+        rewrite unembedEmbed.
+        reflexivity. }
+      rewrite s_eq.
+      reflexivity.
+    - simpl.
+      apply (f_equal2); [ | exact IH ].
+      apply f_equal.
+      rewrite BlackBoxArity.
+      simpl.
+      match goal with
+      |[|- cons _ ?lhs _ _ = cons _ ?rhs _ _] =>
+       assert (s_eq: lhs = rhs)
+      end.
+      { match goal with
+        |[|- _ = Apply S ?erc ] =>
+         assert (ex_s: exists s, erc = embed s); [ eexists; reflexivity | ];
+           rewrite (unembedApply S _ ex_s)
+        end.
+        rewrite <- embedApply.
+        rewrite unembedEmbed.
+        reflexivity. }
+      rewrite s_eq.
+      reflexivity.
+  Qed.
+
+  Definition CL_CoAlgebra:
+      (forall S, WF.WellFormed S -> SigSpec.WellFormed (unembedSubst S)) ->
+      (forall M sigma, {CL Gamma M sigma} + {CL Gamma M sigma -> False}) ->
+      SigmaCoAlgebra Carrier.
+  Proof.
+    intros WF_transport CL_dec.
+    unfold SigmaCoAlgebra.
+    intros s prf.
+    destruct prf as [ M prf ].
+    assert (path_s : Path (blackBoxEmbed s)).
+    { unfold blackBoxEmbed.
+      apply Path_Const.
+      simpl.
+      rewrite BlackBoxArity.
+      simpl.
+      apply PathArgs_cons_arg.
+      fold freeze.
+      apply embed_Path. }
+    generalize (CL_Path_path _ _ _ prf path_s).
+    intro ex_subst.
+    generalize (CL_Path_path_compute_S _ CL_dec _ _ path_s ex_subst).
+    clear ex_subst; intro ex_subst.
+    assert (fully_applied: argumentCount M = arity (rootOf M)).
+    { destruct ex_subst as [ S [ WF_S ex_path ] ].
+      unfold CombinatorSymbol.
+      rewrite <- (source_count_eq (unembedSubst S) (rootOf M)).
+      rewrite unembedApply_c.
+      generalize (ST_organize_ge (Apply S (Gamma (rootOf M)))).
+      rewrite (factorize_organized _ (organize_organized _)).
+      induction ex_path as [ ? ? ? here | ? x xs ].
+      - destruct here as [ path_x [ argCountPrf [ _ tgt_le ] ] ].
+        intro x_ge.
+        rewrite (ST_intersect_nth _ Fin.F1) in x_ge.
+        simpl in x_ge.
+        generalize (Gamma_paths (rootOf M) (unembedSubst S)).
+        rewrite unembedApply_c.
+        intro path_c.
+        generalize (Path_src_count _ _ x_ge path_c path_x).
+        intro src_count_eq'.
+        rewrite src_count_eq'.
+        inversion argCountPrf as [ | n argCountPrf' src_count_eq'' ].
+        + reflexivity.
+        + assert (argCountPrf'' : (Datatypes.S (argumentCount M) <= Datatypes.S n)%nat).
+          { rewrite <- Nat.succ_le_mono.
+            assumption. }
+          rewrite src_count_eq'' in argCountPrf''.
+          generalize (split_path_step _ _ argCountPrf argCountPrf'').
+          intro split_path_eq.
+          rewrite split_path_eq in tgt_le.
+          unfold blackBoxEmbed in tgt_le.
+          assert False; [ | contradiction ].
+          apply (ST_Arrow_Const _ _ _ _ tgt_le).
+      - rewrite (ST_intersect_append_le (cons _ x _ (nil _)) xs).
+        rewrite (ST_InterMeetRight).
+        intro; auto. }
+    apply (mkF _ _ (rootOf M) (unembedSubst (proj1_sig ex_subst)));
+      destruct ex_subst as [ S [ WF_S ex_path ] ].
+    - apply WF_transport; assumption.
+    - generalize (ST_organize_ge (Apply S (Gamma (rootOf M)))).
+      simpl.
+      rewrite (factorize_organized _ (organize_organized (Apply S (Gamma (rootOf M))))).
+      intro root_le.
+      apply nth_F_args.
+      intro k.
+      set (k' := rew <- fully_applied in k).
+      exists (nth (argumentsOf M) k').
+      induction ex_path as [ ? x ? here | ? x xs ? IH ].
+      + destruct here as [ path_x [ argCountPrf [ args_inhab tgt_le ] ] ].
+        eapply CL_ST.
+        * apply (Forall2_nth _ _ _ args_inhab k').
+        * generalize (Gamma_paths (rootOf M) (unembedSubst S)).
+          rewrite unembedApply_c.
+          intro path_c.
+          rewrite (ST_intersect_nth _ Fin.F1) in root_le.
+          assert (argCountPrf' : (argumentCount M <= src_count (Apply S (Gamma (rootOf M))))%nat).
+          { generalize (Path_src_count _ _ root_le path_c path_x).
+            intro count_eq.
+            rewrite count_eq.
+            assumption. }               
+          generalize (Forall2_nth _ _ _ (ST_path_src_n _ _ path_c path_x root_le _ argCountPrf' argCountPrf) k').
+          intro arg_le.
+          rewrite arg_le.
+          unfold Gamma.
+          clear arg_le.
+          revert fully_applied k' argCountPrf'.
+          clear ...
+          intro fully_applied.
+          rewrite fully_applied.
+          unfold eq_rect_r.
+          simpl.
+          clear fully_applied.
+          unfold Gamma.
+          fold CombinatorSymbol in k.
+          fold CombinatorSymbol.
+          induction (domain (rootOf M)) as [ | ? ? ? IH ].
+          { inversion k. }
+          { intro argCountPrf.
+            apply (Fin.caseS' k).
+            - simpl.
+              unfold blackBoxEmbed.
+              simpl.
+              apply (ST_Ax _ _ eq_refl); [ reflexivity | ].
+              rewrite BlackBoxArity.
+              simpl.
+              rewrite unembedApply; [ | eexists; reflexivity ].
+              unfold eq_rect_r.
+              simpl.
+              rewrite unembedEmbed.
+              apply Forall2_cons; [ | apply Forall2_nil ].
+              reflexivity.
+            - intro k'.
+              apply (IH k' (proj2 (Nat.succ_le_mono _ _) argCountPrf)). }
+      + rewrite (ST_intersect_append_le (cons _ x _ (nil _)) xs) in root_le.
+        rewrite (ST_InterMeetRight) in root_le.
+        auto.
+    - assert (source_count_le : (arity (rootOf M) <= src_count (Apply S (Gamma (rootOf M))))%nat).
+      { generalize (source_count_eq (unembedSubst S) (rootOf M)).
+        intro source_count_eq.
+        rewrite unembedApply_c in source_count_eq.
+        unfold CombinatorSymbol.
+        rewrite <- source_count_eq.
+        reflexivity. }
+      assert (split_path_eq:
+                snd (split_path (Apply S (Gamma (rootOf M))) _ source_count_le) =
+                blackBoxEmbed (applySubst (unembedSubst S) (range (rootOf M)))).
+      { clear ...
+        revert source_count_le.
+        generalize (rootOf M).
+        clear M.
+        intros c.
+        unfold Gamma.
+        unfold blackBoxEmbed.
+        fold CombinatorSymbol.
+        induction (domain c) as [ | ? ? ? IH ].
+        - intros; simpl.
+          apply f_equal.
+          rewrite BlackBoxArity.
+          simpl.
+          rewrite unembedApply; [ | eexists; reflexivity ].
+          rewrite unembedEmbed.
+          reflexivity.
+        - simpl.
+          intro source_count_le.
+          generalize (proj2 (PeanoNat.Nat.succ_le_mono _ _) source_count_le).
+          intro source_count_le'.
+          generalize (IH source_count_le').
+          intro IH'.
+          exact IH'. }
+      assert (path_tgt_le:
+                snd (split_path (Apply S (Gamma (rootOf M))) _ source_count_le) <=
+                blackBoxEmbed s).
+      { generalize (ST_organize_ge (Apply S (Gamma (rootOf M)))).
+        rewrite (factorize_organized _ (organize_organized _)).
+        induction ex_path as [ ? ? ? here | ? x xs there IH ].
+        - intro x_ge.
+          rewrite (ST_intersect_nth _ Fin.F1) in x_ge.
+          simpl in x_ge.
+          destruct here as [ path_x [ argCountPrf [ inhab_args x_tgt_le ] ] ].
+          rewrite <- x_tgt_le.
+          generalize (Gamma_paths (rootOf M) (unembedSubst S)).
+          rewrite unembedApply_c.
+          intro path_c.
+          clear split_path_eq inhab_args x_tgt_le.
+          revert fully_applied source_count_le path_c path_x x_ge argCountPrf.
+          clear ...
+          intros fully_applied source_count_le path_c path_x x_ge.
+          rewrite fully_applied.
+          intro argCountPrf.            
+          apply (ST_path_tgt_n _ _ path_c path_x x_ge _ _ argCountPrf).
+        - intro xs_ge.
+          rewrite (ST_intersect_append_le (cons _ x _ (nil _)) xs) in xs_ge.
+          rewrite (ST_InterMeetRight _ _) in xs_ge.
+          exact (IH xs_ge). }
+      rewrite split_path_eq in path_tgt_le.
+      unfold blackBoxEmbed in path_tgt_le.
+      simpl in path_tgt_le.
+      generalize (CI_complete _ _ _ path_tgt_le).
+      intro path_tgt_ci.
+      inversion path_tgt_ci as [ ? ? arity_eq ? args_st [ hd_eq tl_eq ] | | | ].
+      unfold eq_rect_r in args_st.
+      rewrite <- (eq_rect_eq_dec (Nat.eq_dec) _ _ (eq_sym arity_eq)) in args_st.
+      rewrite (vect_exist_eq _ _
+                             (existT_fg_eq (fun x => t IntersectionType x) constructorArity _ _ _ tl_eq))
+        in args_st.
+      rewrite BlackBoxArity in args_st.
+      simpl in args_st.
+      inversion args_st as [ | ? ? ? ? ? arg_st ].
+      generalize (unembed_respectful _ _
+                                     (ex_intro _ _ eq_refl)
+                                     (ex_intro _ _ eq_refl)
+                                     arg_st).
+      intro arg_subsorts.
+      rewrite freezeUnfreeze in arg_subsorts.
+      rewrite freezeUnfreeze in arg_subsorts.
+      rewrite unembedEmbed in arg_subsorts.
+      rewrite unembedEmbed in arg_subsorts.
+      exact arg_subsorts.
+  Defined.
+
+  Definition carrier_eq: forall s s', Carrier s -> Carrier s' -> Prop :=
+    fun s1 s2 c1 c2 => proj1_sig c1 = proj1_sig c2.
+
+  Lemma carrier_eq_refl: forall s c, carrier_eq s s c c.
+  Proof.
+    intros; reflexivity.
+  Qed.
+  Lemma carrier_eq_sym: forall s s' c1 c2, carrier_eq s s' c1 c2 -> carrier_eq s' s c2 c1.
+  Proof.
+    intros; apply eq_sym; assumption.
+  Qed.
+  Lemma carrier_eq_trans: forall s s' s'' c1 c2 c3,
+      carrier_eq s s' c1 c2 -> carrier_eq s' s'' c2 c3 -> carrier_eq s s'' c1 c3.
+  Proof.
+    intros; eapply eq_trans; eassumption.
+  Qed.
+
+  Lemma CL_Algebra_op:
+    forall (WF_transport: forall S, SigSpec.WellFormed S -> WF.WellFormed (embedSubst S)),
+    forall s f, rootOf (proj1_sig (CL_Algebra WF_transport s f)) = op _ _ f.
+  Proof.
+    intros WF_transport s f.
+    unfold CL_Algebra.
+    destruct f as [ op subst wf args tgt_le ].
+    simpl.
+    rewrite (applyAllRoot).
+    reflexivity.
+  Qed.
+  
+  Lemma CL_Algebra_argCount:
+    forall (WF_transport: forall S, SigSpec.WellFormed S -> WF.WellFormed (embedSubst S)),
+    forall s f, argumentCount (proj1_sig (CL_Algebra WF_transport s f)) =
+           (arity (op _ _ f)).
+  Proof.
+    intros WF_transport s f.
+    unfold CL_Algebra.
+    destruct f as [ op subst wf args tgt_le ].
+    simpl.
+    rewrite (applyAllArgumentCount).
+    simpl.
+    rewrite (source_count_eq).
+    reflexivity.
+  Defined.
+
+  Lemma CL_Algebra_args:
+    forall (WF_transport: forall S, SigSpec.WellFormed S -> WF.WellFormed (embedSubst S)),
+    forall s f, argumentsOf (proj1_sig (CL_Algebra WF_transport s f)) =
+           rew <- (CL_Algebra_argCount WF_transport s f) in ProjectTerms _ _ _ (args _ _ f).
+  Proof.
+    intros WF_transport s f.
+    destruct f as [ op subst wf args tgt_le ].       
+    simpl.
+    rewrite (applyAllArguments).
+    simpl.
+    match goal with
+      [|- (rew <- [t Term] ?prf1 in rew <- [t Term] ?prf2 in _) =
+         (rew <- [t Term] ?prf3 in _) ] =>
+      generalize prf2 prf1 prf3
+    end.
+    intro prf1.
+    rewrite prf1.
+    unfold eq_rect_r.
+    simpl.
+    intros prf2 prf3.
+    rewrite (UIP_dec (Nat.eq_dec) prf2 prf3).
+    reflexivity.
+  Qed.
+
+  Lemma CL_CoAlgebra_op:
+    forall (WF_transport: forall S, WF.WellFormed S -> SigSpec.WellFormed (unembedSubst S))
+      (CL_dec: forall M sigma, {CL Gamma M sigma} + {CL Gamma M sigma -> False}),
+    forall s c, op _ _ (CL_CoAlgebra WF_transport  CL_dec s c) = rootOf (proj1_sig c).
+  Proof.
+    intros WF_transport CL_dec s c.
+    destruct c as [ M prf ].
+    reflexivity.
+  Qed.
 (*
+     Lemma CL_CoAlgebra_arity:
+       forall (WellFormed : (Signature.Var -> Sort EmptySet) -> Prop)
+         (WF_transport: forall S, TypeSystem.WellFormed S -> WellFormed (unembedSubst S))
+         (WF_dec: forall S, { TypeSystem.WellFormed S } + { TypeSystem.WellFormed S -> False })
+         (CL_dec: forall M sigma, {CL Gamma M sigma} + {CL Gamma M sigma -> False}),
+       forall s c,
+         arity (op _ _ _ _ _ _ (CL_CoAlgebra WellFormed WF_transport WF_dec CL_dec s c)) =
+         argumentCount (proj1_sig c).
+     Proof.
+       rewrite (sour
+
+     Lemma CL_CoAlgebra_args:
+       forall (WellFormed : (Signature.Var -> Sort EmptySet) -> Prop)
+         (WF_transport: forall S, TypeSystem.WellFormed S -> WellFormed (unembedSubst S))
+         (WF_dec: forall S, { TypeSystem.WellFormed S } + { TypeSystem.WellFormed S -> False })
+         (CL_dec: forall M sigma, {CL Gamma M sigma} + {CL Gamma M sigma -> False}),
+       forall s c, ProjectTerms _ _ _
+                           (args _ _ _ _ _ _
+                                 (CL_CoAlgebra WellFormed WF_transport WF_dec CL_dec s c)) =
+              argumentsOf (proj1_sig c).
+     Proof.
+     argumentsOf (proj1_sig (CL_Algebra WellFormed WF_transport s f)) =
+              rew <- (CL_Algebra_argCount WellFormed WF_transport s f) in ProjectTerms _ _ _ (args _ _ _ _ _ _ f).
+     
+
+     Lemma CL_AlgebraCoAlgebra_inv:
+       forall (WellFormed : (Signature.Var -> Sort EmptySet) -> Prop)
+         (WF_transport1: forall S, WellFormed S -> TypeSystem.WellFormed (embedSubst S))
+         (WF_transport2: forall S, TypeSystem.WellFormed S -> WellFormed (unembedSubst S))
+         (WF_dec: forall S, { TypeSystem.WellFormed S } + { TypeSystem.WellFormed S -> False })
+         (CL_dec: forall M sigma, {CL Gamma M sigma} + {CL Gamma M sigma -> False}),
+       forall s f, F_eq _ _ _ WellFormed _ carrier_eq s f
+                (CL_CoAlgebra WellFormed WF_transport2 WF_dec CL_dec s
+                              (CL_Algebra WellFormed WF_transport1 s f)).
+     Proof.
+       intros WellFormed WF_transport1 WF_transport2 WF_dec CL_dec s f.
+       destruct f as [ op subst WF_subst args tgt_le ].
+       split.
+       - revert args.
+         simpl Top.op at 1.
+         simpl CL_Algebra at 1.
+         set (coalg := fun x => Top.op Sort Signature.Var subsorts WellFormed Carrier s
+                                    (CL_CoAlgebra WellFormed WF_transport2 WF_dec CL_dec s x)).
+         simpl Top.op in coalg.
+         match goal with
+         | [|- _ = Top.op Sort Signature.Var subsorts WellFormed Carrier s (CL_CoAlgebra _ _ _ _ _ ?x) ] =>
+           set (alg := x)
+         end.
+         simpl in alg.
+         revert alg.
+         induction (arity).
+         + simpl in alg.
+ *)
+
+End CombinatoryLogicAlgebra.
+
+
+
+
+
+(* Grave yard
 
 Module Type ProtectedSymbols(SigSpec: CompatibleCLSignature) <: CompatibleCLSignature.
   Definition Sort: Set -> Set := SigSpec.Sort.
@@ -1029,575 +1600,3 @@ Module LiftProperEmbedding
     Instance ProperlyEmbedded: ProperEmbedding.
   End LiftedEmbedding.
 End LiftProperEmbedding. *)
-
-Module CombinatoryLogicAlgebra
-       (Import SigSpec: CompatibleCLSignature)
-       (Import Types: IntersectionTypes(SigSpec))
-       (Import Terms: Terms(SigSpec))
-       (Import ProperEmbedding: WithProperEmbedding(SigSpec)(Types))
-       (Import TypesCountable: CountableTypes(SigSpec)(Types))
-       (Import WF: DecidableWellFormedPredicate(SigSpec)(Types))
-       (Import CL: CombinatoryLogic(SigSpec)(Types)(Terms)(WF))
-       (Import CPL: ComputationalPathLemma(SigSpec)(Types)(Terms)(TypesCountable)(WF)(CL))
-       (Import Alg: Algebraic(SigSpec)).
-  (*Context {UnprotectedConstructorSymbol: Set}.
-  Context `{Signature: `{SignatureSpecification}}.
-  Context `{ContextSymbols: `{SymbolSpecification UnprotectedConstructorSymbol Operation}}.
-  Context `{Embedding: `{ProperEmbedding (ContextSymbols := ProtectedSymbolSpecificationInstance)}}.
-
-  Implicit Types ConstructorSymbol : (unit + UnprotectedConstructorSymbol).
-  Implicit Types VariableSymbol := Var.*)
-  
-  Definition blackBoxEmbedOpen (s: Sort SigSpec.Var): TypeScheme (VariableSymbol := SigSpec.Var) :=
-    ConstScheme BlackBox (rew <- BlackBoxArity in cons _ (embed s) _ (nil _)).
-
-  Definition blackBoxEmbed (s: Sort EmptySet): IntersectionType :=
-    freeze (Skeleton (PT_Const BlackBox (rew <- BlackBoxArity in cons _ (embed s) _ (nil _)))).
-
-  Definition Gamma (c: Operation) :=
-    (fix Gamma_rec n dom :=
-       match dom with
-       | nil _ => blackBoxEmbedOpen (range c)
-       | cons _ param _ params =>
-         ArrowScheme (blackBoxEmbedOpen param) (Gamma_rec _ params)
-       end) _ (domain c).
-  
-  Lemma Gamma_paths:
-    forall (c: Operation) (S: SigSpec.Var -> Sort EmptySet),
-      Path (Apply (embedSubst S) (Gamma c)).
-  Proof.
-    intros c S.
-    unfold Gamma.
-    induction (domain c).
-    - unfold blackBoxEmbedOpen.
-      apply Path_Const.
-      simpl.
-      rewrite BlackBoxArity.
-      simpl.
-      apply PathArgs_cons_arg.
-      fold (Apply).
-      rewrite <- embedApply.
-      apply embed_Path.
-    - apply Path_Arr.
-      assumption.
-  Qed.
-
-  Lemma source_count_eq : forall S op, src_count (Apply (embedSubst S) (Gamma op)) = arity op.
-  Proof.
-    intros S op.
-    unfold Gamma.
-    generalize (arity op) (domain op).
-    intros arity domain.
-    induction domain as [ | ? ? ? IH ].
-    - reflexivity.
-    - simpl.
-      rewrite IH.
-      reflexivity.
-  Qed. 
-
-  Definition Carrier s := { M : Term | CL Gamma M (blackBoxEmbed s) }.
-
-  Definition ProjectTerms: forall S n (args: t (Sort SigSpec.Var) n),
-      F_args Carrier S args -> t Term n :=
-    fun S n args f => 
-      map (fun k => proj1_sig ((F_args_nth _ _ _ f) k)) (positions n).
-
-  Lemma blackBoxEmbed_nth:
-    forall op S k (src_count_eq: src_count (Apply (embedSubst S) (Gamma op)) = arity op),
-      blackBoxEmbed (applySubst S (nth (domain op) (rew <- eq_sym src_count_eq in k))) =
-      nth
-        (fst
-           (split_path (Apply (embedSubst S) (Gamma op)) (src_count (Apply (embedSubst S) (Gamma op)))
-                       (le_n (src_count (Apply (embedSubst S) (Gamma op)))))) k.
-  Proof.
-    intros op S k src_count_eq.
-    generalize (le_n (src_count (Apply (embedSubst S) (Gamma op)))).
-    revert k.
-    generalize src_count_eq.
-    match goal with
-    | [ |- ?tgt ] =>
-      apply (fun x =>
-               rew <- [fun n =>
-                        forall (src_count_eq: n = arity op)
-                          (k: Fin.t n)
-                          (prf: (n <= src_count (Apply (embedSubst S) (Gamma op)))%nat),
-                          blackBoxEmbed (applySubst S (nth (domain op) (rew <- [Fin.t] eq_sym src_count_eq in k))) =
-                          nth (fst (split_path (Apply (embedSubst S) (Gamma op)) n prf)) k]
-                   (src_count_eq) in x)
-    end.
-    clear src_count_eq.
-    intros src_count_eq k prf.
-    unfold eq_rect_r.
-    rewrite <- (eq_rect_eq_dec (Nat.eq_dec) _ _ (eq_sym _)).
-    clear src_count_eq.
-    apply (Forall2_nth (fun x y => blackBoxEmbed (applySubst S x) = y)
-                       (domain op)
-                       (fst (split_path (Apply (embedSubst S) (Gamma op)) (arity op) prf))).
-    clear k.
-    revert prf.
-    unfold Gamma.
-    induction (domain op) as [ | ? ? ? IH ].
-    - intros; apply Forall2_nil.
-    - intro prf. 
-      apply Forall2_cons.
-      + unfold blackBoxEmbed.
-        unfold blackBoxEmbedOpen.
-        simpl.
-        apply f_equal.
-        rewrite BlackBoxArity.
-        simpl.
-        rewrite embedApply.
-        reflexivity.
-      + apply IH.
-  Qed.
-  
-  Definition CL_Algebra:
-      (forall S, SigSpec.WellFormed S -> WF.WellFormed (embedSubst S)) ->
-      SigmaAlgebra Carrier.
-  Proof.
-    unfold SigmaAlgebra.
-    intros WF_transport s Fs.
-    destruct Fs as [ op S WF_S args tgt_le ].
-    assert (opty : CL Gamma (Symbol op) (Apply (embedSubst S) (Gamma op))).
-    { apply CL_Var.
-      apply WF_transport; assumption. }
-    generalize (source_count_eq S op).
-    intro source_count_eq.
-    assert (args' :
-              { Ns: t Term (src_count (Apply (embedSubst S) (Gamma op)))
-              | Forall2 (CL Gamma) Ns (fst (split_path (Apply (embedSubst S) (Gamma op))
-                                                       (src_count (Apply (embedSubst S) (Gamma op)))
-                                                       (le_n _))) }).
-    { exists (rew <- source_count_eq in ProjectTerms _ _ _ args).
-      apply nth_Forall2.
-      unfold eq_rect_r.
-      intro k.
-      assert (rew_ext:
-                (rew [fun n => t Term n] eq_sym source_count_eq in (ProjectTerms S (arity op) (domain op) args)) =
-                rew [t Term] eq_sym source_count_eq in (ProjectTerms S (arity op) (domain op) args)).
-      { rewrite <- (eq_sym source_count_eq).
-        simpl.
-        reflexivity. }
-      rewrite rew_ext.
-      rewrite (nth_k (eq_sym source_count_eq) (ProjectTerms S (arity op) (domain op) args) k).
-      unfold ProjectTerms.
-      rewrite (nth_map _ _ _ _ eq_refl).
-      rewrite (positions_spec).
-      destruct (F_args_nth _ _ _ args (rew <- [Fin.t] eq_sym source_count_eq in k)) as [ M proof ].        
-      simpl.
-      rewrite <- (blackBoxEmbed_nth _ _ _ source_count_eq).
-      assumption. }
-    clear args.
-    assert (tgt_le':
-              snd (split_path (Apply (embedSubst S) (Gamma op))
-                              (src_count (Apply (embedSubst S) (Gamma op)))
-                              (le_n _)) <= blackBoxEmbed s).
-    { unfold blackBoxEmbed.
-      simpl freeze.
-      unfold Gamma.
-      clear args'.
-      generalize (domain op).
-      rewrite <- source_count_eq.
-      clear source_count_eq.
-      intro domain.
-      induction domain as [ | ? ? ? IH ].
-      - simpl.
-        apply (ST_Ax _ _ eq_refl); [ reflexivity | ].
-        rewrite BlackBoxArity.
-        apply Forall2_cons; [ | apply Forall2_nil ].
-        rewrite <- embedApply.
-        apply embed_respectful.
-        assumption.
-      - simpl.
-        match goal with
-        | [ |- (snd (split_path _ _ ?prfSx) <= _)] =>
-          rewrite (split_path_proof_invariant _ _ _ prfSx) in IH
-        end.
-        exact IH. }
-    eexists.
-    eapply CL_ST; [ | apply tgt_le' ].
-    eapply CL_ApplyPath.
-    - apply Gamma_paths. 
-    - eassumption.
-    - exact (proj2_sig args').
-  Defined.
-
-  Lemma unembedApply_c: forall S c,
-      Apply (embedSubst (unembedSubst S)) (Gamma c) =
-      Apply S (Gamma c).
-  Proof.
-    intros S c.
-    unfold Gamma.
-    induction (domain c) as [ | ? ? ? IH ].
-    - unfold blackBoxEmbedOpen.
-      simpl Apply.
-      apply f_equal.
-      rewrite BlackBoxArity.
-      simpl.
-      match goal with
-      |[|- cons _ ?lhs _ _ = cons _ ?rhs _ _] =>
-       assert (s_eq: lhs = rhs)
-      end.
-      { match goal with
-        |[|- _ = Apply S ?erc ] =>
-         assert (ex_s: exists s, erc = embed s); [ eexists; reflexivity | ];
-           rewrite (unembedApply S _ ex_s)
-        end.
-        rewrite <- embedApply.
-        rewrite unembedEmbed.
-        reflexivity. }
-      rewrite s_eq.
-      reflexivity.
-    - simpl.
-      apply (f_equal2); [ | exact IH ].
-      apply f_equal.
-      rewrite BlackBoxArity.
-      simpl.
-      match goal with
-      |[|- cons _ ?lhs _ _ = cons _ ?rhs _ _] =>
-       assert (s_eq: lhs = rhs)
-      end.
-      { match goal with
-        |[|- _ = Apply S ?erc ] =>
-         assert (ex_s: exists s, erc = embed s); [ eexists; reflexivity | ];
-           rewrite (unembedApply S _ ex_s)
-        end.
-        rewrite <- embedApply.
-        rewrite unembedEmbed.
-        reflexivity. }
-      rewrite s_eq.
-      reflexivity.
-  Qed.
-
-  Definition CL_CoAlgebra:
-      (forall S, WF.WellFormed S -> SigSpec.WellFormed (unembedSubst S)) ->
-      (forall M sigma, {CL Gamma M sigma} + {CL Gamma M sigma -> False}) ->
-      SigmaCoAlgebra Carrier.
-  Proof.
-    intros WF_transport CL_dec.
-    unfold SigmaCoAlgebra.
-    intros s prf.
-    destruct prf as [ M prf ].
-    assert (path_s : Path (blackBoxEmbed s)).
-    { unfold blackBoxEmbed.
-      apply Path_Const.
-      simpl.
-      rewrite BlackBoxArity.
-      simpl.
-      apply PathArgs_cons_arg.
-      fold freeze.
-      apply embed_Path. }
-    generalize (CL_Path_path _ _ _ prf path_s).
-    intro ex_subst.
-    generalize (CL_Path_path_compute_S _ CL_dec _ _ path_s ex_subst).
-    clear ex_subst; intro ex_subst.
-    assert (fully_applied: argumentCount M = arity (rootOf M)).
-    { destruct ex_subst as [ S [ WF_S ex_path ] ].
-      unfold CombinatorSymbol.
-      rewrite <- (source_count_eq (unembedSubst S) (rootOf M)).
-      rewrite unembedApply_c.
-      generalize (ST_organize_ge (Apply S (Gamma (rootOf M)))).
-      rewrite (factorize_organized _ (organize_organized _)).
-      induction ex_path as [ ? ? ? here | ? x xs ].
-      - destruct here as [ path_x [ argCountPrf [ _ tgt_le ] ] ].
-        intro x_ge.
-        rewrite (ST_intersect_nth _ Fin.F1) in x_ge.
-        simpl in x_ge.
-        generalize (Gamma_paths (rootOf M) (unembedSubst S)).
-        rewrite unembedApply_c.
-        intro path_c.
-        generalize (Path_src_count _ _ x_ge path_c path_x).
-        intro src_count_eq'.
-        rewrite src_count_eq'.
-        inversion argCountPrf as [ | n argCountPrf' src_count_eq'' ].
-        + reflexivity.
-        + assert (argCountPrf'' : (Datatypes.S (argumentCount M) <= Datatypes.S n)%nat).
-          { rewrite <- Nat.succ_le_mono.
-            assumption. }
-          rewrite src_count_eq'' in argCountPrf''.
-          generalize (split_path_step _ _ argCountPrf argCountPrf'').
-          intro split_path_eq.
-          rewrite split_path_eq in tgt_le.
-          unfold blackBoxEmbed in tgt_le.
-          assert False; [ | contradiction ].
-          apply (ST_Arrow_Const _ _ _ _ tgt_le).
-      - rewrite (ST_intersect_append_le (cons _ x _ (nil _)) xs).
-        rewrite (ST_InterMeetRight).
-        intro; auto. }
-    apply (mkF _ _ (rootOf M) (unembedSubst (proj1_sig ex_subst)));
-      destruct ex_subst as [ S [ WF_S ex_path ] ].
-    - apply WF_transport; assumption.
-    - generalize (ST_organize_ge (Apply S (Gamma (rootOf M)))).
-      simpl.
-      rewrite (factorize_organized _ (organize_organized (Apply S (Gamma (rootOf M))))).
-      intro root_le.
-      apply nth_F_args.
-      intro k.
-      set (k' := rew <- fully_applied in k).
-      exists (nth (argumentsOf M) k').
-      induction ex_path as [ ? x ? here | ? x xs ? IH ].
-      + destruct here as [ path_x [ argCountPrf [ args_inhab tgt_le ] ] ].
-        eapply CL_ST.
-        * apply (Forall2_nth _ _ _ args_inhab k').
-        * generalize (Gamma_paths (rootOf M) (unembedSubst S)).
-          rewrite unembedApply_c.
-          intro path_c.
-          rewrite (ST_intersect_nth _ Fin.F1) in root_le.
-          assert (argCountPrf' : (argumentCount M <= src_count (Apply S (Gamma (rootOf M))))%nat).
-          { generalize (Path_src_count _ _ root_le path_c path_x).
-            intro count_eq.
-            rewrite count_eq.
-            assumption. }               
-          generalize (Forall2_nth _ _ _ (ST_path_src_n _ _ path_c path_x root_le _ argCountPrf' argCountPrf) k').
-          intro arg_le.
-          rewrite arg_le.
-          unfold Gamma.
-          clear arg_le.
-          revert fully_applied k' argCountPrf'.
-          clear ...
-          intro fully_applied.
-          rewrite fully_applied.
-          unfold eq_rect_r.
-          simpl.
-          clear fully_applied.
-          unfold Gamma.
-          fold CombinatorSymbol in k.
-          fold CombinatorSymbol.
-          induction (domain (rootOf M)) as [ | ? ? ? IH ].
-          { inversion k. }
-          { intro argCountPrf.
-            apply (Fin.caseS' k).
-            - simpl.
-              unfold blackBoxEmbed.
-              simpl.
-              apply (ST_Ax _ _ eq_refl); [ reflexivity | ].
-              rewrite BlackBoxArity.
-              simpl.
-              rewrite unembedApply; [ | eexists; reflexivity ].
-              unfold eq_rect_r.
-              simpl.
-              rewrite unembedEmbed.
-              apply Forall2_cons; [ | apply Forall2_nil ].
-              reflexivity.
-            - intro k'.
-              apply (IH k' (proj2 (Nat.succ_le_mono _ _) argCountPrf)). }
-      + rewrite (ST_intersect_append_le (cons _ x _ (nil _)) xs) in root_le.
-        rewrite (ST_InterMeetRight) in root_le.
-        auto.
-    - assert (source_count_le : (arity (rootOf M) <= src_count (Apply S (Gamma (rootOf M))))%nat).
-      { generalize (source_count_eq (unembedSubst S) (rootOf M)).
-        intro source_count_eq.
-        rewrite unembedApply_c in source_count_eq.
-        unfold CombinatorSymbol.
-        rewrite <- source_count_eq.
-        reflexivity. }
-      assert (split_path_eq:
-                snd (split_path (Apply S (Gamma (rootOf M))) _ source_count_le) =
-                blackBoxEmbed (applySubst (unembedSubst S) (range (rootOf M)))).
-      { clear ...
-        revert source_count_le.
-        generalize (rootOf M).
-        clear M.
-        intros c.
-        unfold Gamma.
-        unfold blackBoxEmbed.
-        fold CombinatorSymbol.
-        induction (domain c) as [ | ? ? ? IH ].
-        - intros; simpl.
-          apply f_equal.
-          rewrite BlackBoxArity.
-          simpl.
-          rewrite unembedApply; [ | eexists; reflexivity ].
-          rewrite unembedEmbed.
-          reflexivity.
-        - simpl.
-          intro source_count_le.
-          generalize (proj2 (PeanoNat.Nat.succ_le_mono _ _) source_count_le).
-          intro source_count_le'.
-          generalize (IH source_count_le').
-          intro IH'.
-          exact IH'. }
-      assert (path_tgt_le:
-                snd (split_path (Apply S (Gamma (rootOf M))) _ source_count_le) <=
-                blackBoxEmbed s).
-      { generalize (ST_organize_ge (Apply S (Gamma (rootOf M)))).
-        rewrite (factorize_organized _ (organize_organized _)).
-        induction ex_path as [ ? ? ? here | ? x xs there IH ].
-        - intro x_ge.
-          rewrite (ST_intersect_nth _ Fin.F1) in x_ge.
-          simpl in x_ge.
-          destruct here as [ path_x [ argCountPrf [ inhab_args x_tgt_le ] ] ].
-          rewrite <- x_tgt_le.
-          generalize (Gamma_paths (rootOf M) (unembedSubst S)).
-          rewrite unembedApply_c.
-          intro path_c.
-          clear split_path_eq inhab_args x_tgt_le.
-          revert fully_applied source_count_le path_c path_x x_ge argCountPrf.
-          clear ...
-          intros fully_applied source_count_le path_c path_x x_ge.
-          rewrite fully_applied.
-          intro argCountPrf.            
-          apply (ST_path_tgt_n _ _ path_c path_x x_ge _ _ argCountPrf).
-        - intro xs_ge.
-          rewrite (ST_intersect_append_le (cons _ x _ (nil _)) xs) in xs_ge.
-          rewrite (ST_InterMeetRight _ _) in xs_ge.
-          exact (IH xs_ge). }
-      rewrite split_path_eq in path_tgt_le.
-      unfold blackBoxEmbed in path_tgt_le.
-      simpl in path_tgt_le.
-      generalize (CI_complete _ _ _ path_tgt_le).
-      intro path_tgt_ci.
-      inversion path_tgt_ci as [ ? ? arity_eq ? args_st [ hd_eq tl_eq ] | | | ].
-      unfold eq_rect_r in args_st.
-      rewrite <- (eq_rect_eq_dec (Nat.eq_dec) _ _ (eq_sym arity_eq)) in args_st.
-      rewrite (vect_exist_eq _ _
-                             (existT_fg_eq (fun x => t IntersectionType x) constructorArity _ _ _ tl_eq))
-        in args_st.
-      rewrite BlackBoxArity in args_st.
-      simpl in args_st.
-      inversion args_st as [ | ? ? ? ? ? arg_st ].
-      generalize (unembed_respectful _ _
-                                     (ex_intro _ _ eq_refl)
-                                     (ex_intro _ _ eq_refl)
-                                     arg_st).
-      intro arg_subsorts.
-      rewrite freezeUnfreeze in arg_subsorts.
-      rewrite freezeUnfreeze in arg_subsorts.
-      rewrite unembedEmbed in arg_subsorts.
-      rewrite unembedEmbed in arg_subsorts.
-      exact arg_subsorts.
-  Defined.
-
-  Definition carrier_eq: forall s s', Carrier s -> Carrier s' -> Prop :=
-    fun s1 s2 c1 c2 => proj1_sig c1 = proj1_sig c2.
-
-  Lemma carrier_eq_refl: forall s c, carrier_eq s s c c.
-  Proof.
-    intros; reflexivity.
-  Qed.
-  Lemma carrier_eq_sym: forall s s' c1 c2, carrier_eq s s' c1 c2 -> carrier_eq s' s c2 c1.
-  Proof.
-    intros; apply eq_sym; assumption.
-  Qed.
-  Lemma carrier_eq_trans: forall s s' s'' c1 c2 c3,
-      carrier_eq s s' c1 c2 -> carrier_eq s' s'' c2 c3 -> carrier_eq s s'' c1 c3.
-  Proof.
-    intros; eapply eq_trans; eassumption.
-  Qed.
-
-  Lemma CL_Algebra_op:
-    forall (WF_transport: forall S, SigSpec.WellFormed S -> WF.WellFormed (embedSubst S)),
-    forall s f, rootOf (proj1_sig (CL_Algebra WF_transport s f)) = op _ _ f.
-  Proof.
-    intros WF_transport s f.
-    unfold CL_Algebra.
-    destruct f as [ op subst wf args tgt_le ].
-    simpl.
-    rewrite (applyAllRoot).
-    reflexivity.
-  Qed.
-  
-  Lemma CL_Algebra_argCount:
-    forall (WF_transport: forall S, SigSpec.WellFormed S -> WF.WellFormed (embedSubst S)),
-    forall s f, argumentCount (proj1_sig (CL_Algebra WF_transport s f)) =
-           (arity (op _ _ f)).
-  Proof.
-    intros WF_transport s f.
-    unfold CL_Algebra.
-    destruct f as [ op subst wf args tgt_le ].
-    simpl.
-    rewrite (applyAllArgumentCount).
-    simpl.
-    rewrite (source_count_eq).
-    reflexivity.
-  Defined.
-
-  Lemma CL_Algebra_args:
-    forall (WF_transport: forall S, SigSpec.WellFormed S -> WF.WellFormed (embedSubst S)),
-    forall s f, argumentsOf (proj1_sig (CL_Algebra WF_transport s f)) =
-           rew <- (CL_Algebra_argCount WF_transport s f) in ProjectTerms _ _ _ (args _ _ f).
-  Proof.
-    intros WF_transport s f.
-    destruct f as [ op subst wf args tgt_le ].       
-    simpl.
-    rewrite (applyAllArguments).
-    simpl.
-    match goal with
-      [|- (rew <- [t Term] ?prf1 in rew <- [t Term] ?prf2 in _) =
-         (rew <- [t Term] ?prf3 in _) ] =>
-      generalize prf2 prf1 prf3
-    end.
-    intro prf1.
-    rewrite prf1.
-    unfold eq_rect_r.
-    simpl.
-    intros prf2 prf3.
-    rewrite (UIP_dec (Nat.eq_dec) prf2 prf3).
-    reflexivity.
-  Qed.
-
-  Lemma CL_CoAlgebra_op:
-    forall (WF_transport: forall S, WF.WellFormed S -> SigSpec.WellFormed (unembedSubst S))
-      (CL_dec: forall M sigma, {CL Gamma M sigma} + {CL Gamma M sigma -> False}),
-    forall s c, op _ _ (CL_CoAlgebra WF_transport  CL_dec s c) = rootOf (proj1_sig c).
-  Proof.
-    intros WF_transport CL_dec s c.
-    destruct c as [ M prf ].
-    reflexivity.
-  Qed.
-(*
-     Lemma CL_CoAlgebra_arity:
-       forall (WellFormed : (Signature.Var -> Sort EmptySet) -> Prop)
-         (WF_transport: forall S, TypeSystem.WellFormed S -> WellFormed (unembedSubst S))
-         (WF_dec: forall S, { TypeSystem.WellFormed S } + { TypeSystem.WellFormed S -> False })
-         (CL_dec: forall M sigma, {CL Gamma M sigma} + {CL Gamma M sigma -> False}),
-       forall s c,
-         arity (op _ _ _ _ _ _ (CL_CoAlgebra WellFormed WF_transport WF_dec CL_dec s c)) =
-         argumentCount (proj1_sig c).
-     Proof.
-       rewrite (sour
-
-     Lemma CL_CoAlgebra_args:
-       forall (WellFormed : (Signature.Var -> Sort EmptySet) -> Prop)
-         (WF_transport: forall S, TypeSystem.WellFormed S -> WellFormed (unembedSubst S))
-         (WF_dec: forall S, { TypeSystem.WellFormed S } + { TypeSystem.WellFormed S -> False })
-         (CL_dec: forall M sigma, {CL Gamma M sigma} + {CL Gamma M sigma -> False}),
-       forall s c, ProjectTerms _ _ _
-                           (args _ _ _ _ _ _
-                                 (CL_CoAlgebra WellFormed WF_transport WF_dec CL_dec s c)) =
-              argumentsOf (proj1_sig c).
-     Proof.
-     argumentsOf (proj1_sig (CL_Algebra WellFormed WF_transport s f)) =
-              rew <- (CL_Algebra_argCount WellFormed WF_transport s f) in ProjectTerms _ _ _ (args _ _ _ _ _ _ f).
-     
-
-     Lemma CL_AlgebraCoAlgebra_inv:
-       forall (WellFormed : (Signature.Var -> Sort EmptySet) -> Prop)
-         (WF_transport1: forall S, WellFormed S -> TypeSystem.WellFormed (embedSubst S))
-         (WF_transport2: forall S, TypeSystem.WellFormed S -> WellFormed (unembedSubst S))
-         (WF_dec: forall S, { TypeSystem.WellFormed S } + { TypeSystem.WellFormed S -> False })
-         (CL_dec: forall M sigma, {CL Gamma M sigma} + {CL Gamma M sigma -> False}),
-       forall s f, F_eq _ _ _ WellFormed _ carrier_eq s f
-                (CL_CoAlgebra WellFormed WF_transport2 WF_dec CL_dec s
-                              (CL_Algebra WellFormed WF_transport1 s f)).
-     Proof.
-       intros WellFormed WF_transport1 WF_transport2 WF_dec CL_dec s f.
-       destruct f as [ op subst WF_subst args tgt_le ].
-       split.
-       - revert args.
-         simpl Top.op at 1.
-         simpl CL_Algebra at 1.
-         set (coalg := fun x => Top.op Sort Signature.Var subsorts WellFormed Carrier s
-                                    (CL_CoAlgebra WellFormed WF_transport2 WF_dec CL_dec s x)).
-         simpl Top.op in coalg.
-         match goal with
-         | [|- _ = Top.op Sort Signature.Var subsorts WellFormed Carrier s (CL_CoAlgebra _ _ _ _ _ ?x) ] =>
-           set (alg := x)
-         end.
-         simpl in alg.
-         revert alg.
-         induction (arity).
-         + simpl in alg.
- *)
-
-End CombinatoryLogicAlgebra.
