VarianceLabeledTree.v
@@ -1,0 +1,645 @@
+Require Import Coq.Arith.PeanoNat.
+Require Import Coq.Vectors.Fin.
+Require Import Coq.Vectors.Vector.
+Require Import Coq.Classes.RelationClasses.
+Require Import Coq.Logic.Eqdep_dec.
+Require Import Coq.Init.Wf.
+Require Import Coq.Arith.Wf_nat.
+
+Require Import VectorQuantification.
+
+Import EqNotations.
+
+Inductive Variance := Co | Contra | In.
+
+Class LabelInfo (Label: Set) :=
+  { labelArity : Label -> nat;
+    successorVariance: forall (l: Label), Fin.t (labelArity l) -> Variance }.
+
+Inductive VLTree (Label: Set) `{LabelInfo Label} (Var: Set): Set :=
+| Node : forall (l: Label), t (VLTree Label Var) (labelArity l) -> VLTree Label Var
+| Hole : Var -> VLTree Label Var.
+
+Inductive VLTreeOrder (Label: Set) (LOrder: Label -> Label -> Prop) `{LabelInfo Label}:
+  VLTree Label False -> VLTree Label False -> Prop :=
+| NodesOrdered:
+    forall l1 l2
+      (arityEq: labelArity l1 = labelArity l2)
+      (varianceEq: forall k, successorVariance l1 k = successorVariance l2 (rew arityEq in k))
+      xs ys,
+      LOrder l1 l2 ->
+      VLForestOrder Label LOrder
+                    (map (successorVariance l1) (positions (labelArity l1)))
+                    xs (rew <- arityEq in ys) ->
+      VLTreeOrder Label LOrder (Node _ _ l1 xs) (Node _ _ l2 ys)
+with VLForestOrder (Label: Set) (LOrder: Label -> Label -> Prop) `{LabelInfo Label}:
+       forall {n : nat}, t Variance n -> t (VLTree Label False) n -> t (VLTree Label False) n -> Prop :=
+     | VLForestOrder_empty: VLForestOrder Label LOrder (nil _) (nil _) (nil _)
+     | VLForestOrder_cons_co:
+         forall x y n (vs : t Variance n) xs ys,
+           VLTreeOrder Label LOrder x y ->
+           VLForestOrder Label LOrder vs xs ys ->
+           VLForestOrder Label LOrder (cons _ Co _ vs) (cons _ x _ xs) (cons _ y _ ys)
+     | VLForestOrder_cons_contra:
+         forall x y n (vs : t Variance n) xs ys,
+           VLTreeOrder Label LOrder y x ->
+           VLForestOrder Label LOrder vs xs ys ->
+           VLForestOrder Label LOrder (cons _ Contra _ vs) (cons _ x _ xs) (cons _ y _ ys)
+     | VLForestOrder_cons_in:
+         forall x y n (vs : t Variance n) xs ys,
+           VLTreeOrder Label LOrder x y ->
+           VLTreeOrder Label LOrder y x ->
+           VLForestOrder Label LOrder vs xs ys ->
+           VLForestOrder Label LOrder (cons _ In _ vs) (cons _ x _ xs) (cons _ y _ ys).
+
+Definition Variance_eq_dec (v1: Variance): forall v2, { v1 = v2 } + { v1 <> v2 } :=
+  match v1 as v1' return forall v2, { v1' = v2 } + { v1' <> v2 } with
+  | Co =>
+    fun v2 =>
+      match v2 with
+      | Co => left (eq_refl Co)
+      | _ => right (fun eq => eq_ind Co (fun y => match y with | Co => True | _ => False end) I _ eq)
+      end
+  | Contra =>
+    fun v2 =>
+      match v2 with
+      | Contra => left (eq_refl Contra)
+      | _ => right (fun eq => eq_ind Contra (fun y => match y with | Contra => True | _ => False end) I _ eq)
+      end
+  | In =>
+    fun v2 =>
+      match v2 with
+      | In => left (eq_refl In)
+      | _ => right (fun eq => eq_ind In (fun y => match y with | In => True | _ => False end) I _ eq)
+      end
+  end.
+
+Fixpoint VLTree_rect' (Label: Set) (info: LabelInfo Label) (Var: Set) (P: VLTree Label Var -> Type)
+         (IHVar: forall x, P (Hole _ _ x)) 
+         (IH: forall (l: Label) (successors: t (VLTree Label Var) (labelArity l)),
+             ForAll' P successors -> P (Node _ _ l successors))
+         (tree: VLTree Label Var): P tree :=
+  match tree with
+  | Node _ _ l successors =>
+    IH l _
+       ((fix successor_rect (n: nat) (successors: t (VLTree Label Var) n): ForAll' P successors :=
+           match successors with
+           | nil _ => ForAll'_nil _
+           | cons _ x n xs =>
+             ForAll'_cons P _ _ (VLTree_rect' Label info Var P IHVar IH x) (successor_rect n xs)
+           end) _ successors)
+  | Hole _ _ x => IHVar x
+  end.
+
+Definition Tree_eq_dec (Label: Set) `{LabelInfo Label} (Var: Set)
+      (Label_eq_dec: forall (l1 l2: Label), { l1 = l2 } + { l1 <> l2 })
+      (Var_eq_dec: forall (alpha beta: Var), { alpha = beta } + { alpha <> beta }):
+  forall (t1 t2: VLTree Label Var), { t1 = t2 } + { t1 <> t2 }.
+Proof.
+  intro t1.
+  induction t1 as [ alpha | l1 ts1 IH ] using VLTree_rect'.
+  - intro t2.
+    destruct t2 as [ l2 ts2 | beta ].
+    + right; intro devil; inversion devil.
+    + destruct (Var_eq_dec alpha beta) as [ var_eq | not_var_eq ].
+      * left; rewrite var_eq; reflexivity.
+      * right; intro devil; inversion devil; contradiction.
+  - intro t2.
+    destruct t2 as [ l2 ts2 | beta ].
+    + destruct (Label_eq_dec l1 l2) as [ label_eq | not_label_eq ];
+        [ | right; intro devil; inversion devil; contradiction ].
+      revert ts2.
+      rewrite <- label_eq.
+      clear label_eq.
+      intro ts2.
+      assert (children_eq_dec: { ts1 = ts2 } + { ts1 <> ts2 }).
+      { induction IH as [ | ? ? ? prf prfs IH' ].
+        - apply (fun r => case0 (fun xs => { _ = xs } + { _ <> xs }) r ts2).
+          left; reflexivity.
+        - apply (caseS' ts2); clear ts2; intros y ys.
+          destruct (prf y) as [ y_eq | not_y_eq ];
+            [ | right; intro devil; inversion devil; contradiction ].
+          destruct (IH' ys) as [ ys_eq | not_ys_eq ].
+          + left; rewrite y_eq; rewrite ys_eq; reflexivity.
+          + right; intro devil.
+            inversion devil as [ [ y_eq' ys_eq ] ].
+            apply not_ys_eq.
+            apply (vect_exist_eq _ _ ys_eq). }
+      destruct children_eq_dec as [ children_eq | not_children_eq ].
+      * left; rewrite children_eq; reflexivity.
+      * right; intro devil.
+        inversion devil as [ ts_eq ].
+        apply not_children_eq.
+        apply (vect_exist_eq _ _ (existT_fg_eq (t (VLTree Label Var)) labelArity _ _ _ ts_eq)).
+    + right; intro devil; inversion devil.
+Defined.
+
+Fixpoint VLTree_size (Label: Set) `{LabelInfo Label} (Var: Set) (t: VLTree Label Var): nat :=
+  match t with
+  | Node _ _ _ xs =>
+    S (fold_right (fun t max => Nat.max (VLTree_size _ _ t) max) xs 0)
+  | Hole _ _ _  => 1
+  end.
+
+Lemma VLTree_size_lt (Label: Set) `{LabelInfo Label} (Var: Set):
+  forall (l : Label) (xs: t (VLTree Label Var) (labelArity l)),
+    Forall (fun t => VLTree_size _ _ t < VLTree_size _ _ (Node _ _ l xs)) xs.
+Proof.
+  intro l.
+  simpl.
+  generalize (labelArity l).
+  intros n xs.
+  induction xs as [ | x n xs IH ].
+  - apply Forall_nil.
+  - apply Forall_cons.
+    + simpl.
+      unfold "_ < _".
+      rewrite <- (Nat.succ_le_mono).
+      apply (Nat.le_max_l).
+    + apply nth_Forall.
+      intro k.
+      generalize (Forall_nth _ _ IH k).
+      simpl.
+      unfold "_ < _".
+      rewrite <- (Nat.succ_le_mono).
+      rewrite <- (Nat.succ_le_mono). 
+      intro prf.
+      rewrite prf.
+      apply (Nat.le_max_r).
+Qed.
+      
+      
+Fixpoint substitute {Label Var Var': Set} `{LabelInfo Label}
+         (f : Var -> VLTree Label Var') (tree: VLTree Label Var): VLTree Label Var' :=
+  match tree with
+  | Node _ _ l successors => Node _ _ l (map (substitute f) successors)
+  | Hole _ _ x => f x
+  end.
+
+Section VLOrderDec.
+  Variable (Label: Set).
+  Variable (LOrder: Label -> Label -> Prop).
+  Variable (LOrder_dec: forall l1 l2, {LOrder l1 l2} + {LOrder l1 l2 -> False}).
+  Context `{LabelInfo Label}.
+  Context `{PreOrder _ LOrder}.
+  
+  Section VLForestOrderDec.
+    Variable max_size: nat.
+    Variable VLTreeOrder_dec: forall t1 t2,
+      max (VLTree_size _ _ t1) (VLTree_size _ _ t2) < max_size ->
+      { VLTreeOrder Label LOrder t1 t2 } + { VLTreeOrder Label LOrder t1 t2 -> False }.
+    Fixpoint VLForestOrder_dec
+             {n: nat} (variances: t Variance n) (xs ys: t (VLTree Label False) n) {struct xs}:
+      Forall (fun x => VLTree_size _ _ x < max_size) xs ->
+      Forall (fun y => VLTree_size _ _ y < max_size) ys ->
+      { VLForestOrder Label LOrder variances xs ys } + { VLForestOrder Label LOrder variances xs ys -> False }.
+    Proof.  
+      revert variances ys.
+      case xs as [ | x n xs ].
+      - intros variances ys.
+        apply (fun r => case0 (fun vs => _ -> _ -> { VLForestOrder Label LOrder vs _ _ } +
+                                           { VLForestOrder Label LOrder vs _ _ -> False})
+                           r variances).
+        apply (fun r => case0 (fun ys => _ -> _ -> { VLForestOrder Label LOrder _ _ ys } +
+                                           { VLForestOrder Label LOrder _ _ ys -> False})
+                           r ys).
+        intros.
+        left.
+        apply VLForestOrder_empty.
+      - intros variances ys.
+        apply (caseS' variances); clear variances; intros variance variances.
+        apply (caseS' ys); clear ys; intros y ys.
+        intros xsok ysok.
+        assert (xok: VLTree_size _ _ x < max_size).
+        { inversion xsok; assumption. }
+        assert (yok: VLTree_size _ _ y < max_size).
+        { inversion ysok; assumption. }
+        assert (xyok: max (VLTree_size _ _ x) (VLTree_size _ _ y) < max_size).
+        { apply Nat.max_lub_lt; assumption. }
+        assert (yxok: max (VLTree_size _ _ y) (VLTree_size _ _ x) < max_size).
+        { rewrite Nat.max_comm; assumption. }
+        generalize (append_Forall2 _ (cons _ x _ (nil _)) xs xsok); clear xsok; intro xsok.
+        generalize (append_Forall2 _ (cons _ y _ (nil _)) ys ysok); clear ysok; intro ysok.
+        destruct variance.
+        + destruct (VLTreeOrder_dec x y xyok) as [ xy | not_xy ].
+          * destruct (VLForestOrder_dec _ variances xs ys xsok ysok) as [ | not_xsys ].
+            { left; apply VLForestOrder_cons_co; assumption. }
+            { right; intro devil; inversion devil as [
+                                                    | ? ? ? ? ? ? ? prfs n_eq [ vs_eq ] [ x_eq xs_eq ] [ y_eq ys_eq ]
+                                                    | | ].
+              apply not_xsys.
+              rewrite (vect_exist_eq _ _ vs_eq) in prfs.
+              rewrite (vect_exist_eq _ _ xs_eq) in prfs.
+              rewrite (vect_exist_eq _ _ ys_eq) in prfs.
+              assumption. }
+          * right; intro devil; inversion devil; contradiction.
+        + destruct (VLTreeOrder_dec y x yxok) as [ yx | not_yx ].
+          * destruct (VLForestOrder_dec _ variances xs ys xsok ysok) as [ | not_xsys ].
+            { left; apply VLForestOrder_cons_contra; assumption. }
+            { right; intro devil; inversion devil as [ |
+                                                       | ? ? ? ? ? ? ? prfs n_eq [ vs_eq ] [ x_eq xs_eq ] [ y_eq ys_eq ]
+                                                       | ].
+              apply not_xsys.
+              rewrite (vect_exist_eq _ _ vs_eq) in prfs.
+              rewrite (vect_exist_eq _ _ xs_eq) in prfs.
+              rewrite (vect_exist_eq _ _ ys_eq) in prfs.
+              assumption. }
+          * right; intro devil; inversion devil; contradiction.
+        + destruct (VLTreeOrder_dec x y xyok) as [ xy | not_xy ];
+            destruct (VLTreeOrder_dec y x yxok) as [ yx | not_yx ];
+            try solve [ right; intro devil; inversion devil; contradiction ].
+          destruct (VLForestOrder_dec _ variances xs ys xsok ysok) as [ | not_xsys ].
+          * left; apply VLForestOrder_cons_in; assumption.
+          * right; intro devil; inversion devil as [ |
+                                                     |
+                                                     | ? ? ? ? ? ? ? ? prfs n_eq
+                                                         [ vs_eq ] [ x_eq xs_eq ] [ y_eq ys_eq ]
+                                                   ].
+            apply not_xsys.
+            rewrite (vect_exist_eq _ _ vs_eq) in prfs.
+            rewrite (vect_exist_eq _ _ xs_eq) in prfs.
+            rewrite (vect_exist_eq _ _ ys_eq) in prfs.
+            assumption.
+    Defined.
+  End VLForestOrderDec.
+
+  Definition VLTreeOrder_dec_step
+             (t1 t2: VLTree Label False)
+             (VLTreeOrder_dec_rec:
+                forall t1' t2',
+                  max (VLTree_size _ _ t1') (VLTree_size _ _ t2') < max (VLTree_size _ _ t1) (VLTree_size _ _ t2) ->
+                  { VLTreeOrder Label LOrder t1' t2' } + { VLTreeOrder Label LOrder t1' t2' -> False }):    
+    { VLTreeOrder Label LOrder t1 t2 } + { VLTreeOrder Label LOrder t1 t2 -> False }.
+  Proof.
+    case t1 as [ l1 ts1 | ]; [ | contradiction ].
+    case t2 as [ l2 ts2 | ]; [ | contradiction ].
+    assert (ts1_lt:
+              Forall (fun x => VLTree_size _ _ x < max (VLTree_size _ _ (Node _ _ l1 ts1))
+                                                    (VLTree_size _ _ (Node _ _ l2 ts2)))
+                     ts1).
+    { apply nth_Forall.
+      intro k.
+      generalize (Forall_nth _ _ (VLTree_size_lt _ _ l1 ts1) k).
+      unfold "_ < _".
+      intro prf.
+      rewrite prf.
+      apply Nat.le_max_l. }
+    assert (ts2_lt:
+              Forall (fun y => VLTree_size _ _ y < max (VLTree_size _ _ (Node _ _ l1 ts1))
+                                                    (VLTree_size _ _ (Node _ _ l2 ts2)))
+                     ts2).
+    { apply nth_Forall.
+      intro k.
+      generalize (Forall_nth _ _ (VLTree_size_lt _ _ l2 ts2) k).
+      unfold "_ < _".
+      intro prf.
+      rewrite prf.
+      apply Nat.le_max_r. }    
+    destruct (Nat.eq_dec (labelArity l1) (labelArity l2))
+      as [ arityEq | ];
+      [ | right; intro devil; inversion devil; contradiction ].
+    assert (varianceEq: { forall k, successorVariance l1 k = successorVariance l2 (rew arityEq in k) } +
+                        { (forall k, successorVariance l1 k = successorVariance l2 (rew arityEq in k)) -> False }).
+    { destruct (Vector_eq_dec Variance_eq_dec
+                              (map (successorVariance l1) (positions (labelArity l1)))
+                              (rew <- [t Variance] arityEq in (map (successorVariance l2)
+                                                                  (positions (labelArity l2)))))
+        as [ eq | ineq ].
+      - left.
+        intro k.
+        generalize (f_equal (fun xs => nth xs k) eq).
+        rewrite (nth_map _ _ _ _ eq_refl).
+        unfold eq_rect_r.
+        rewrite (nth_k).
+        rewrite (nth_map _ _ _ _ eq_refl).
+        rewrite positions_spec.
+        rewrite positions_spec.
+        assert (eq_sym_eq: forall n m (eq: n = m) (k: Fin.t n), rew <- [Fin.t] eq_sym eq in k = rew eq in k).
+        { intros n m.
+          unfold eq_rect_r.
+          destruct n; destruct m; intro eq'; inversion eq' as [ eq'' ].
+          - intro k'.
+            rewrite <- (eq_rect_eq_dec (Nat.eq_dec) _ _ eq').
+            rewrite <- (eq_rect_eq_dec (Nat.eq_dec) _ _ (eq_sym (eq_sym eq'))).
+            reflexivity.
+          - revert eq'.
+            rewrite eq''.
+            intro eq'.
+            intro k'.
+            rewrite <- (eq_rect_eq_dec (Nat.eq_dec) _ _ eq').
+            rewrite <- (eq_rect_eq_dec (Nat.eq_dec) _ _ (eq_sym (eq_sym eq'))).
+            reflexivity. }
+        rewrite eq_sym_eq.
+        intro; assumption.
+      - right; intro devil.
+        apply ineq.
+        revert devil.
+        clear ...
+        generalize (successorVariance l1).
+        intro succVar.
+        generalize (successorVariance l2).
+        intro succVar2.
+        unfold eq_rect_r.
+        destruct (labelArity l1) as [ | m ]; destruct (labelArity l2) as [ | n ];
+          try solve [ inversion arityEq ].
+        + rewrite <- (eq_rect_eq_dec (Nat.eq_dec) _ _ (eq_sym arityEq)).
+          intros; reflexivity.
+        + inversion arityEq as [ arityEq' ].
+          revert arityEq succVar.
+          rewrite arityEq'.
+          intro arityEq.
+          rewrite <- (eq_rect_eq_dec (Nat.eq_dec) _ _ (eq_sym arityEq)).
+          intros succVar succVarEq'.
+          assert (succVarEq: forall k, succVar k = succVar2 k).
+          { intro k.
+            generalize (succVarEq' k).
+            rewrite <- (eq_rect_eq_dec (Nat.eq_dec) _ _ arityEq).
+            intro; assumption. }
+          revert succVarEq.
+          clear ...
+          revert succVar succVar2.
+          induction n as [ | n IH ].
+          * intros; simpl.
+            rewrite (succVarEq F1).
+            reflexivity.
+          * intros succVar succVar2 succVarEq.
+            simpl.
+            rewrite (succVarEq F1).
+            apply f_equal.
+            generalize (IH (fun k => succVar (FS k)) (fun k => succVar2 (FS k))
+                           (fun k => succVarEq (FS k))).
+            rewrite (map_fg).
+            rewrite (map_fg _ succVar2).
+            simpl; intro; assumption. }
+    inversion varianceEq as [ varianceEq' | varianceInEq ].
+    - destruct (LOrder_dec l1 l2) as [ l1l2 | ]; [ | right; intro devil; inversion devil; contradiction ].
+      rewrite <- (rewrite_vect _ (eq_sym arityEq) ts2) in ts2_lt.
+      fold (eq_rect_r (t (VLTree Label False)) ts2 arityEq) in ts2_lt.
+      generalize (VLForestOrder_dec _ VLTreeOrder_dec_rec
+                    (map (successorVariance l1) (positions (labelArity l1)))
+                    ts1 (rew <- arityEq in ts2)
+                    ts1_lt ts2_lt).
+      intro successor_dec.
+      inversion successor_dec as [ ts1ts2 | not_ts1ts2 ].
+      + left; eapply NodesOrdered; eassumption.
+      + right; intro devil.
+        inversion devil as [ ? ? ? ? ? ? ? prfs [ l1_eq ts1_eq ]  [ l2_eq ts2_eq ] ].
+        apply not_ts1ts2.
+        rewrite (vect_exist_eq _ _ (existT_fg_eq (t (VLTree Label False)) labelArity l1 _ _ ts1_eq)) in prfs.
+        rewrite (vect_exist_eq _ _ (existT_fg_eq (t (VLTree Label False)) labelArity l2 _ _ ts2_eq)) in prfs.
+        rewrite (UIP_dec (Nat.eq_dec) _ arityEq) in prfs.
+        exact prfs.
+    - right; intro devil.
+      inversion devil as [ ? ? arityEq' varianceEq'' ].
+      apply varianceInEq.
+      intro k.
+      generalize (varianceEq'' k).
+      rewrite (UIP_dec (Nat.eq_dec)  arityEq arityEq').
+      intro; assumption.
+  Defined.
+
+  Lemma WF_VLTree_size_max:
+    well_founded (fun (xy x'y': VLTree Label False * VLTree Label False) =>
+                    max (VLTree_size _ _ (fst xy)) (VLTree_size _ _ (snd xy)) <
+                    max (VLTree_size _ _ (fst x'y')) (VLTree_size _ _ (snd x'y'))).
+  Proof.
+    apply well_founded_ltof.
+  Qed.   
+  
+  Definition VLTreeOrder_dec (t1 t2: VLTree Label False):
+    { VLTreeOrder Label LOrder t1 t2 } + { VLTreeOrder Label LOrder t1 t2 -> False } :=
+    Fix_F_2 _ VLTreeOrder_dec_step (WF_VLTree_size_max (t1, t2)).
+End VLOrderDec.
+
+Instance VLOrderRefl (Label: Set) (LOrder: Label -> Label -> Prop)
+         `{LabelInfo Label}
+         `{Reflexive _ LOrder}: Reflexive (VLTreeOrder Label LOrder).
+Proof.
+  unfold Reflexive.
+  intro tree.
+  induction tree as [ alpha | l ts IH ] using VLTree_rect';
+    [ contradiction | ].
+  apply (NodesOrdered _ _ l l eq_refl).
+  - simpl; intro k; reflexivity.
+  - reflexivity.
+  - unfold eq_rect_r.
+    simpl.
+    revert ts IH.
+    generalize (map (successorVariance l) (positions (labelArity l))).
+    generalize (labelArity l).
+    clear ...
+    intros n variances ts IH.
+    induction IH as [ | t n ts prf prfs IH ].
+    + apply (fun r => case0 (fun vs => VLForestOrder _ _ vs _ _) r variances).
+      apply VLForestOrder_empty.
+    + apply (caseS' variances); clear variances; intros variance variances.
+      destruct variance.
+      * apply VLForestOrder_cons_co; auto.
+      * apply VLForestOrder_cons_contra; auto.
+      * apply VLForestOrder_cons_in; auto.
+Qed.
+
+
+Lemma VLTree_size_order
+      (Label: Set) (LOrder: Label -> Label -> Prop)
+      `{LabelInfo Label}:
+  forall t1 t2, VLTreeOrder Label LOrder t1 t2 -> VLTree_size _ _ t1 = VLTree_size _ _ t2.
+Proof.
+  intros t1 t2.
+  apply (fun tgt =>
+           @Fix_F_2 _ _ (fun x y => max (VLTree_size _ _ (fst x)) (VLTree_size _ _ (snd x)) <
+                                 max (VLTree_size _ _ (fst y)) (VLTree_size _ _ (snd y)))
+                    (fun x y => VLTreeOrder Label LOrder x y -> VLTree_size Label False x = VLTree_size Label False y)
+                    tgt t1 t2 (WF_VLTree_size_max _ (t1, t2))).
+  clear t1 t2.
+  intros t1 t2 IH.
+  destruct t1 as [ l1 ts1 | alpha];
+    [ | intro devil; inversion devil ];
+    destruct t2 as [ l2 ts2 | beta ];
+    [ | intro devil; inversion devil ].
+  simpl.
+  intro orderprf.
+  inversion orderprf as [ ? ? arityEq varianceEq ? ? labelOrder forestOrder  [ l1_eq ts1_eq ] [ l2_eq ts2_eq ]].
+  rewrite (vect_exist_eq _ _ (existT_fg_eq (t (VLTree Label False)) (labelArity) _ _ _ ts1_eq)) in forestOrder.
+  rewrite (vect_exist_eq _ _ (existT_fg_eq (t (VLTree Label False)) (labelArity) _ _ _ ts2_eq)) in forestOrder.
+  apply f_equal.
+  generalize (VLTree_size_lt _ _ l1 ts1).
+  generalize (VLTree_size_lt _ _ l2 ts2).
+  clear orderprf ts1_eq ts2_eq varianceEq.
+  revert ts1 arityEq ts2 IH forestOrder.
+  clear ...
+  simpl.
+  generalize (map (successorVariance l1) (positions (labelArity l1))).
+  generalize (labelArity l1).
+  intros n variances ts1 arityEq.
+  rewrite <- arityEq.
+  clear arityEq.
+  intros ts2 IH orderprf ts2ok ts1ok.
+  assert (argSizeEq: Forall2 (fun x y => VLTree_size Label False x = VLTree_size Label False y) ts1 ts2).
+  { apply nth_Forall2.
+    intro k.
+    assert (kthorder: (VLTreeOrder _ LOrder (nth ts1 k) (nth ts2 k)) \/
+                      (VLTreeOrder _ LOrder (nth ts2 k) (nth ts1 k))).
+    { revert orderprf.
+      clear ...
+      induction k as [ | n k IH ].
+      - apply (caseS' ts1); clear ts1; intros t1 ts1.
+        apply (caseS' ts2); clear ts2; intros t2 ts2.
+        intro orderprf.
+        simpl.
+        inversion orderprf; solve [ left; assumption | right; assumption ].
+      - apply (caseS' ts1); clear ts1; intros t1 ts1.
+        apply (caseS' ts2); clear ts2; intros t2 ts2.
+        apply (caseS' variances); clear variances; intros variance variances.
+        simpl.
+        intro orderprf.
+        inversion orderprf as [
+                             | ? ? ? ? ? ? ? prfs n_eq [ v_eq vs_eq ] [ l1_eq ts1_eq ] [l2_eq ts2_eq ]
+                             | ? ? ? ? ? ? ? prfs n_eq [ v_eq vs_eq ] [ l1_eq ts1_eq ] [l2_eq ts2_eq ]
+                             | ? ? ? ? ? ? ? ? prfs n_eq [ v_eq vs_eq ] [ l1_eq ts1_eq ] [l2_eq ts2_eq ] ];
+          rewrite (vect_exist_eq _ _ vs_eq) in prfs;
+          rewrite (vect_exist_eq _ _ ts1_eq) in prfs;
+          rewrite (vect_exist_eq _ _ ts2_eq) in prfs;
+          eapply IH; eassumption. }
+    destruct kthorder.
+    - apply IH.
+      + unfold "_ < _".
+        apply (proj1 (Nat.succ_le_mono _ _ )).
+        apply (Nat.max_le_compat).
+        * apply (proj2 (Nat.succ_le_mono _ _) (Forall_nth _ _ ts1ok k)).
+        * apply (proj2 (Nat.succ_le_mono _ _) (Forall_nth _ _ ts2ok k)).
+      +  assumption.
+    - apply eq_sym.
+      apply IH.
+      + unfold "_ < _".
+        apply (proj1 (Nat.succ_le_mono _ _ )).
+        rewrite (Nat.max_comm _ _).
+        apply (Nat.max_le_compat).
+        * apply (proj2 (Nat.succ_le_mono _ _) (Forall_nth _ _ ts1ok k)).
+        * apply (proj2 (Nat.succ_le_mono _ _) (Forall_nth _ _ ts2ok k)).
+      + assumption. }
+  revert argSizeEq.
+  clear ...
+  intro argSizeEq.
+  induction argSizeEq as [ | n t1 t2 ts1 ts2 hd_eq IH ].
+  - reflexivity.
+  - simpl.
+    rewrite hd_eq.
+    apply f_equal.
+    assumption.
+Qed.
+
+
+(* TODO: *)
+Instance VLOrderTrans (Label: Set) (LOrder: Label -> Label -> Prop)
+         `{LabelInfo Label}
+         `{Transitive _ LOrder}: Transitive (VLTreeOrder Label LOrder).
+Proof.
+  unfold Transitive.
+  intro t1.
+  destruct t1 as [ l1 ts1 | alpha];
+    [ | intros ? ? devil; inversion devil ].
+  - intros t2 t3 t1t2 t2t3. 
+    inversion t1t2 as [ ? l2 arityEq12 varianceEq12 ? ts2 lOrder12 forestOrder12 [ t1_eq ts1_eq ] [ t2_eq ] ].
+    rewrite (vect_exist_eq _ _ (existT_fg_eq _ _ _ _ _ ts1_eq)) in forestOrder12.
+    clear ts1_eq xs.
+    inversion t2t3 as [ l2' l3 arityEq23 varianceEq23 ts2' ts3 lOrder23 forestOrder23 [ t2_eq' ] [ t3_eq ]].
+    rewrite <- t2_eq' in t2_eq.
+    inversion t2_eq as [ [ l2_eq ts2_eq ] ].
+    clear t2_eq t2_eq'.
+    assert (arityEq23' : labelArity l2 = labelArity l3).
+    { rewrite l2_eq; assumption. }
+    assert (varianceEq23' : forall k : Fin.t (labelArity l2),
+               successorVariance l2 k = successorVariance l3 (rew [Fin.t] arityEq23' in k)).
+    { revert varianceEq23.
+      revert l2_eq.
+      clear ...
+      intro l2_eq.
+      revert arityEq23'.
+      rewrite l2_eq.
+      intros arityEq23'.
+      rewrite (UIP_dec (Nat.eq_dec) arityEq23' arityEq23).
+      intro; assumption. }
+    assert (lOrder23': LOrder l2 l3).
+    { rewrite l2_eq; assumption. }
+    assert (forestOrder23':
+              VLForestOrder Label LOrder (map (successorVariance l2) (positions (labelArity l2))) ts2
+                            (rew <- [t (VLTree Label False)] arityEq23' in ts3)).
+    { clear varianceEq23' varianceEq23 forestOrder12.
+      revert l2_eq ts2 ts2' ts2_eq arityEq23 arityEq23' forestOrder23.
+      clear ...
+      intro l2_eq.
+      rewrite l2_eq.
+      intros ts2 ts2' ts2_eq.
+      rewrite (vect_exist_eq _ _ (existT_fg_eq (t (VLTree Label False)) (labelArity) _ _ _ ts2_eq)).
+      intros arityEq23 arityEq23'.
+      rewrite (UIP_dec (Nat.eq_dec) arityEq23 arityEq23').
+      intros; assumption. }
+    clear t1t2 t2t3 arityEq23 varianceEq23 forestOrder23 t3_eq ts2_eq.
+    revert arityEq23' arityEq12 ts1 ts2 ts3 varianceEq12 varianceEq23' forestOrder12 forestOrder23'.
+    clear ...
+    generalize (successorVariance l2).
+    induction (labelArity l2).
+    + admit.
+    + 
+    
+    intro  arityEq12.
+    
+    rewrite <- arityEq12.
+    unfold eq_rect_r at 1.
+    simpl.
+    clear arityEq12.
+    
+    induction (labelArity l1).
+    
+    intros succVar_l2 arityEq23.
+    revert succVar_l2.
+    generalize (successorVariance l3).
+    intro succVar_l3.
+    
+    rewrite <- arityEq23.
+    
+    
+    apply (NodesOrdered _ _ l1 l3 (eq_trans arityEq12 arityEq23')).
+    + intro k.
+      rewrite (eq_trans (varianceEq12 k) (varianceEq23' (rew arityEq12 in k))).
+      apply f_equal.
+      clear ...
+      rewrite <- arityEq23'.
+      simpl.
+      rewrite <- arityEq12.
+      simpl.
+      reflexivity.
+    + transitivity l2; assumption.
+    + clear ts2_eq.
+      revert arityEq23' ts2 forestOrder12 forestOrder23' varianceEq12 varianceEq23'.
+      clear ...
+      generalize (successorVariance l2).
+      rewrite <- arityEq12.
+      unfold eq_rect_r.
+      simpl.
+      intros succVar2 arityEq23'.
+      generalize (successorVariance l3).
+      revert ts3.
+      rewrite <- arityEq23'.
+      simpl.
+      intros ts3 succVar3 ts2  forestOrder12 forestOrder23 succVar2_eq succVar3_eq.
+      assert (varEq: map (successorVariance l1) (positions (labelArity l1)) =
+                     map succVar2 (positions (labelArity l1))).
+      { apply map_extensional.
+        intro k.
+        rewrite (succVar2_eq k).
+        reflexivity. }
+      rewrite <- varEq in forestOrder23.
+      revert ts1 ts2 ts3 forestOrder12 forestOrder23.
+      clear ...
+      generalize (map (successorVariance l1)).
+      intros forestOrder12.
+      revert 
+      induction forestOrder12.
+      * intros; assumption.
+      * apply (caseS' ts3); clear ts3; intros t3 ts3.
+        intros forestOrder23 IH.
+        inversion forestOrder23 as [ | ? ? ? ? ? ? prf prfs n_eq [ var_eq ] [ y_eq ys_eq ] [ t3_eq ts3_eq ] | | ].
+        apply VLForestOrder_cons_Co.
+*)
